@@ -1,0 +1,2304 @@
+From stdpp Require Export pmap gmap decidable.
+From TensorRocq Require Import SizedGraph.Definitions HyperGraph Aux_pos Syntax Aux_stdpp.
+
+
+Section StackCompose.
+
+
+  Context {N T : Type}.
+
+Lemma relabel_stack_sized_graphs_aux {n m n' m'} (scohg : SizedCospanHyperGraph N T n m)
+  (scohg' : SizedCospanHyperGraph N T n' m') f {Hf : Inj eq eq f} :
+  relabel_sized_graph f (stack_sized_graphs_aux scohg scohg') =
+  stack_sized_graphs_aux (relabel_sized_graph f scohg) (relabel_sized_graph f scohg').
+Proof.
+  apply scohg_ext; [apply relabel_stack_graphs_aux|].
+  cbn.
+  rewrite (kmap_union f); done.
+Qed.
+
+
+Lemma stack_sized_graphs_relabel {n m n' m'} (scohg : SizedCospanHyperGraph N T n m)
+  (scohg' : SizedCospanHyperGraph N T n' m') ft fb {Hft : Inj eq eq ft} {Hfb : Inj eq eq fb} :
+  stack_sized_graphs (relabel_sized_graph ft scohg) (relabel_sized_graph fb scohg') =
+  relabel_sized_graph (pos_map ft fb) (stack_sized_graphs scohg scohg').
+Proof.
+  unfold stack_sized_graphs.
+  rewrite relabel_stack_sized_graphs_aux by apply _.
+  rewrite 2 reindex_relabel_sized_graph, 4 relabel_sized_graph_compose by apply _.
+  done.
+Qed.
+
+Lemma reindex_stack_sized_graphs_aux {n m n' m'} (scohg : SizedCospanHyperGraph N T n m)
+  (scohg' : SizedCospanHyperGraph N T n' m') f `{Hf : !Inj eq eq f} :
+  reindex_sized_graph f (stack_sized_graphs_aux scohg scohg') =
+  stack_sized_graphs_aux (reindex_sized_graph f scohg) (reindex_sized_graph f scohg').
+Proof.
+  apply scohg_ext; [|done..].
+  now apply reindex_stack_graphs_aux.
+Qed.
+
+Lemma stack_sized_graphs_reindex {n m n' m'} (scohg : SizedCospanHyperGraph N T n m)
+  (scohg' : SizedCospanHyperGraph N T n' m') ft fb
+  `{Hft : !Inj eq eq ft, Hfb : !Inj eq eq fb} :
+  stack_sized_graphs (reindex_sized_graph ft scohg) (reindex_sized_graph fb scohg') =
+  reindex_sized_graph (pos_map ft fb) (stack_sized_graphs scohg scohg').
+Proof.
+  unfold stack_sized_graphs.
+  rewrite (reindex_stack_sized_graphs_aux _ _ _).
+  rewrite 2 reindex_relabel_sized_graph, 4 (reindex_sized_graph_compose _ _).
+  done.
+Qed.
+
+#[export] Instance stack_sized_graphs_sized_isomorphic {n m n' m'} :
+  Proper (sized_isomorphic ==> sized_isomorphic ==> sized_isomorphic)
+    (@stack_sized_graphs N T n m n' m').
+Proof.
+  intros scohg1 scohg1' (fv1 & fe1 & Hfv1 & Hfe1 & ->)%sized_isomorphic_exists
+    scohg2 scohg2' (fv2 & fe2 & Hfv2 & Hfe2 & ->)%sized_isomorphic_exists.
+  rewrite stack_sized_graphs_relabel, (stack_sized_graphs_reindex _ _ _ _) by apply _.
+  apply (sized_iso_relabel_reindex _ _ _).
+Qed.
+
+(* FIXME: Move *)
+
+#[export] Instance stack_graphs_cohg_vert_eq_Proper {n m n' m'} :
+  Proper (cohg_vert_eq ==> cohg_vert_eq ==> cohg_vert_eq)
+    (@stack_graphs T n m n' m').
+Proof.
+  intros scohg1 scohg1' Heq1 scohg2 scohg2' Heq2.
+  unfold cohg_vert_eq in *.
+  rewrite 2 norm_verts_stack_graphs.
+  now f_equal.
+Qed.
+
+#[export] Instance swapped_stack_graphs_cohg_vert_eq_Proper {n m n' m'} :
+  Proper (cohg_vert_eq ==> cohg_vert_eq ==> cohg_vert_eq)
+    (@swapped_stack_graphs T n m n' m').
+Proof.
+  intros scohg1 scohg1' Heq1 scohg2 scohg2' Heq2.
+  unfold cohg_vert_eq in *.
+  rewrite 2 norm_verts_swapped_stack_graphs.
+  now f_equal.
+Qed.
+
+
+#[export] Instance stack_sized_graphs_scohg_vert_eq_Proper {n m n' m'} :
+  Proper (scohg_vert_eq ==> scohg_vert_eq ==> scohg_vert_eq)
+    (@stack_sized_graphs N T n m n' m').
+Proof.
+  intros scohg1 scohg1' Heq1 scohg2 scohg2' Heq2.
+  split; [now apply stack_graphs_cohg_vert_eq_Proper; [apply Heq1.1|apply Heq2.1]|].
+  change (vertices _) with (vertices (stack_graphs scohg1 scohg2)).
+  rewrite vertices_stack_graphs.
+  apply proj2 in Heq1, Heq2.
+  cbn.
+  intros v.
+  rewrite 2 lookup_union.
+  rewrite elem_of_union.
+  intros [(k & -> & Hk)%elem_of_map|(k & -> & Hk)%elem_of_map];
+  rewrite 2 (lookup_kmap _), 2 (lookup_kmap_None _ _ _).2,
+    2?(left_id_L None _), 2?(right_id_L None _) by lia; auto.
+Qed.
+
+#[export] Instance stack_sized_graphs_struct_sized_isomorphic_Proper {n m n' m'} :
+  Proper (struct_sized_isomorphic ==> struct_sized_isomorphic ==> struct_sized_isomorphic)
+    (@stack_sized_graphs N T n m n' m').
+Proof.
+  apply proper_struct_sized_isomorphic_of_vert_eq_binary.
+  - apply _.
+  - intros ? ? ? ? ? ?.
+    now apply stack_sized_graphs_sized_isomorphic.
+Qed.
+
+
+Lemma stack_sized_graphs_struct_sized_isomorphic {n m n' m'} (scohg1 scohg1' : SizedCospanHyperGraph N T n m)
+  (scohg2 scohg2' : SizedCospanHyperGraph N T n' m') :
+  scohg1 ≡ᵢ scohg1' -> scohg2 ≡ᵢ scohg2' ->
+  stack_sized_graphs scohg1 scohg2 ≡ᵢ stack_sized_graphs scohg1' scohg2'.
+Proof.
+  now intros; apply stack_sized_graphs_struct_sized_isomorphic_Proper.
+Qed.
+
+
+Lemma relabel_swapped_stack_sized_graphs_aux {n m n' m'} (scohg : SizedCospanHyperGraph N T n m)
+  (scohg' : SizedCospanHyperGraph N T n' m') f {Hf : Inj eq eq f} :
+  relabel_sized_graph f (swapped_stack_sized_graphs_aux scohg scohg') =
+  swapped_stack_sized_graphs_aux (relabel_sized_graph f scohg) (relabel_sized_graph f scohg').
+Proof.
+  apply scohg_ext; [apply relabel_swapped_stack_graphs_aux|].
+  cbn.
+  rewrite (kmap_union f); done.
+Qed.
+
+Lemma swapped_stack_sized_graphs_relabel {n m n' m'} (scohg : SizedCospanHyperGraph N T n m)
+  (scohg' : SizedCospanHyperGraph N T n' m') ft fb {Hft : Inj eq eq ft} {Hfb : Inj eq eq fb} :
+  swapped_stack_sized_graphs (relabel_sized_graph ft scohg) (relabel_sized_graph fb scohg') =
+  relabel_sized_graph (pos_map ft fb) (swapped_stack_sized_graphs scohg scohg').
+Proof.
+  unfold swapped_stack_sized_graphs.
+  rewrite relabel_swapped_stack_sized_graphs_aux by apply _.
+  rewrite 2 reindex_relabel_sized_graph, 4 relabel_sized_graph_compose by apply _.
+  done.
+Qed.
+
+Lemma reindex_swapped_stack_sized_graphs_aux {n m n' m'} (scohg : SizedCospanHyperGraph N T n m)
+  (scohg' : SizedCospanHyperGraph N T n' m') f `{Hf : !Inj eq eq f} :
+  reindex_sized_graph f (swapped_stack_sized_graphs_aux scohg scohg') =
+  swapped_stack_sized_graphs_aux (reindex_sized_graph f scohg) (reindex_sized_graph f scohg').
+Proof.
+  apply scohg_ext; [apply reindex_swapped_stack_graphs_aux, _|done].
+Qed.
+
+Lemma swapped_stack_sized_graphs_reindex {n m n' m'} (scohg : SizedCospanHyperGraph N T n m)
+  (scohg' : SizedCospanHyperGraph N T n' m') ft fb
+  `{Hft : !Inj eq eq ft, Hfb : !Inj eq eq fb} :
+  swapped_stack_sized_graphs (reindex_sized_graph ft scohg) (reindex_sized_graph fb scohg') =
+  reindex_sized_graph (pos_map ft fb) (swapped_stack_sized_graphs scohg scohg').
+Proof.
+  unfold swapped_stack_sized_graphs.
+  rewrite (reindex_swapped_stack_sized_graphs_aux _ _ _) by apply _.
+  rewrite 2 reindex_relabel_sized_graph, 4 (reindex_sized_graph_compose _ _) by apply _.
+  done.
+Qed.
+
+Lemma swapped_stack_sized_graphs_sized_isomorphic {n m n' m'} (scohg1 scohg1' : SizedCospanHyperGraph N T n m)
+  (scohg2 scohg2' : SizedCospanHyperGraph N T n' m') :
+  sized_isomorphic scohg1 scohg1' -> sized_isomorphic scohg2 scohg2' ->
+  sized_isomorphic (swapped_stack_sized_graphs scohg1 scohg2) (swapped_stack_sized_graphs scohg1' scohg2').
+Proof.
+  intros (fv1 & fe1 & Hfv1 & Hfe1 & ->)%sized_isomorphic_exists
+    (fv2 & fe2 & Hfv2 & Hfe2 & ->)%sized_isomorphic_exists.
+  rewrite swapped_stack_sized_graphs_relabel, (swapped_stack_sized_graphs_reindex _ _ _ _) by apply _.
+  apply (sized_iso_relabel_reindex _ _ _).
+Qed.
+
+
+#[export] Instance swapped_stack_sized_graphs_scohg_vert_eq_Proper {n m n' m'} :
+  Proper (scohg_vert_eq ==> scohg_vert_eq ==> scohg_vert_eq)
+    (@swapped_stack_sized_graphs N T n m n' m').
+Proof.
+  intros scohg1 scohg1' Heq1 scohg2 scohg2' Heq2.
+  split; [now apply swapped_stack_graphs_cohg_vert_eq_Proper; [apply Heq1.1|apply Heq2.1]|].
+  change (vertices _) with (vertices (swapped_stack_graphs scohg1 scohg2)).
+  rewrite vertices_swapped_stack_graphs.
+  apply proj2 in Heq1, Heq2.
+  cbn.
+  intros v.
+  rewrite 2 lookup_union.
+  rewrite elem_of_union.
+  intros [(k & -> & Hk)%elem_of_map|(k & -> & Hk)%elem_of_map];
+  rewrite 2 (lookup_kmap _), 2 (lookup_kmap_None _ _ _).2,
+    2?(left_id_L None _), 2?(right_id_L None _) by lia; auto.
+Qed.
+
+Lemma swapped_stack_sized_graphs_struct_sized_isomorphic_Proper {n m n' m'} :
+  Proper (struct_sized_isomorphic ==> struct_sized_isomorphic ==> struct_sized_isomorphic)
+    (@swapped_stack_sized_graphs N T n m n' m').
+Proof.
+  apply proper_struct_sized_isomorphic_of_vert_eq_binary.
+  - apply _.
+  - intros ? ? ? ? ? ?.
+    now apply swapped_stack_sized_graphs_sized_isomorphic.
+Qed.
+
+
+Lemma swapped_stack_sized_graphs_struct_sized_isomorphic {n m n' m'} (scohg1 scohg1' : SizedCospanHyperGraph N T n m)
+  (scohg2 scohg2' : SizedCospanHyperGraph N T n' m') :
+  scohg1 ≡ᵢ scohg1' -> scohg2 ≡ᵢ scohg2' ->
+  swapped_stack_sized_graphs scohg1 scohg2 ≡ᵢ swapped_stack_sized_graphs scohg1' scohg2'.
+Proof.
+  now intros; apply swapped_stack_sized_graphs_struct_sized_isomorphic_Proper.
+Qed.
+
+Lemma sized_add_top_loop_relabel_sized_graph {n m} f `{Hf : !Inj eq eq f} (scohg : SizedCospanHyperGraph N T (S n) (S m)) :
+  sized_add_top_loop (relabel_sized_graph f scohg) =
+  relabel_sized_graph f (sized_add_top_loop scohg).
+Proof.
+  apply scohg_ext; [apply (add_top_loop_relabel_graph _)|].
+  cbn.
+  unfold map_relabel_one.
+  rewrite (kmap_partial_alter _).
+  rewrite 2 vhd_vmap.
+  rewrite (lookup_kmap f).
+  done.
+Qed.
+
+Lemma sized_add_top_loop_reindex_sized_graph {n m} f (scohg : SizedCospanHyperGraph N T (S n) (S m)) :
+  sized_add_top_loop (reindex_sized_graph f scohg) =
+  reindex_sized_graph f (sized_add_top_loop scohg).
+Proof.
+  apply scohg_ext; [apply (add_top_loop_reindex_graph f)|done].
+Qed.
+
+Lemma vertices_add_top_loop_subset {n m } (cohg : CospanHyperGraph T (S n) (S m)) :
+  vertices (add_top_loop cohg) ⊆ vertices cohg.
+Proof.
+  unfold add_top_loop.
+  rewrite vertices_relabel_graph.
+  rewrite set_map_fn_singleton_L.
+  destruct cohg as [hg ins outs].
+  cbn.
+  inv_all_vec_fin.
+  cbn.
+  rewrite 2 vertices_vertices_hg_decomp; cbn -[union].
+  rewrite 2 list_to_set_app_L.
+  cbn -[union].
+  rewrite vertices_hg_add_vertices.
+  apply union_least; [apply subseteq_union_r; set_solver +|].
+  case_decide; set_solver +.
+Qed.
+
+
+
+Lemma norm_sized_verts_sized_add_top_loop {n m} (scohg : SizedCospanHyperGraph N T (S n) (S m)) :
+  norm_sized_verts (sized_add_top_loop scohg) =
+  norm_sized_verts (sized_add_top_loop (norm_sized_verts scohg)).
+Proof.
+  apply scohg_ext; [apply norm_verts_add_top_loop|].
+  cbn.
+  rewrite <- (vertices_norm_verts (add_top_loop (norm_verts scohg))).
+  rewrite <- norm_verts_add_top_loop.
+  rewrite vertices_norm_verts.
+  apply map_eq.
+  intros k.
+  rewrite 2 map_lookup_filter.
+  cbn.
+  case_guard; cbn; [rewrite 2 bind_with_Some|unfold mbind, option_bind; now repeat case_match].
+  rewrite 2 lookup_map_relabel_one.
+  rewrite fn_lookup_singleton_case.
+  case_decide; [subst|].
+  - pose proof (vertices_add_top_loop_subset scohg).
+    rewrite map_lookup_filter.
+    cbn.
+    enough (vhd scohg.(outputs) ∈ vertices scohg) by (
+      case_guard; cbn; [now rewrite bind_with_Some|
+      unfold mbind, option_bind; now repeat case_match]).
+    rewrite vertices_vertices_hg_decomp, list_to_set_app_L.
+    inv_vec (outputs scohg); cbn -[union]; set_solver +.
+  - rewrite map_lookup_filter.
+    cbn.
+    enough (k ∈ vertices scohg) by (
+      case_guard; cbn; [now rewrite bind_with_Some|
+      unfold mbind, option_bind; now repeat case_match]).
+    now apply vertices_add_top_loop_subset.
+Qed.
+
+Lemma norm_sized_verts_idemp {n m} (scohg : SizedCospanHyperGraph N T n m) :
+  norm_sized_verts (norm_sized_verts scohg) = norm_sized_verts scohg.
+Proof.
+  apply scohg_ext; [apply norm_verts_idemp|].
+  cbn.
+  rewrite map_filter_filter.
+  apply map_filter_ext.
+  cbn.
+  rewrite vertices_norm_verts.
+  tauto.
+Qed.
+
+Lemma norm_sized_verts_sized_add_top_loops {n m o} (scohg : SizedCospanHyperGraph N T (n + m) (n + o)) :
+  norm_sized_verts (sized_add_top_loops scohg) = norm_sized_verts (sized_add_top_loops (norm_sized_verts scohg)).
+Proof.
+  induction n; [cbn; now rewrite norm_sized_verts_idemp|].
+  cbn.
+  now rewrite IHn, norm_sized_verts_sized_add_top_loop, <- IHn.
+Qed.
+
+#[export] Instance sized_add_top_loop_proper {n m} :
+  Proper (@scohg_vert_eq N T (S n) (S m) ==> scohg_vert_eq) sized_add_top_loop.
+Proof.
+  intros cohg cohg' Heq.
+  rewrite <- norm_sized_verts_vert_eq.
+  rewrite norm_sized_verts_sized_add_top_loop.
+  rewrite (norm_sized_verts_of_vert_eq _ _ Heq).
+  rewrite <- norm_sized_verts_sized_add_top_loop.
+  rewrite norm_sized_verts_vert_eq.
+  done.
+Qed.
+
+
+Lemma sized_add_top_loop_struct_sized_isomorphic {n m} (scohg scohg' : SizedCospanHyperGraph N T (S n) (S m)) :
+  scohg ≡ᵢ scohg' ->
+  sized_add_top_loop scohg ≡ᵢ sized_add_top_loop scohg'.
+Proof.
+  intros (fv & fe & Hfv & Hfe & Heq)%sized_isomorphic_exists.
+  rewrite <- norm_sized_verts_vert_eq, norm_sized_verts_sized_add_top_loop.
+  rewrite <- (norm_sized_verts_vert_eq (sized_add_top_loop scohg')),
+    (norm_sized_verts_sized_add_top_loop scohg').
+  rewrite Heq.
+  rewrite (sized_add_top_loop_relabel_sized_graph _), sized_add_top_loop_reindex_sized_graph.
+  rewrite (norm_sized_verts_vert_eq (sized_add_top_loop _)),
+    (norm_sized_verts_vert_eq (relabel_sized_graph _ _)).
+  apply (subrel' sized_isomorphic).
+  now constructor.
+Qed.
+
+Definition relabel_sized_graph_one {n m} (k k' : positive) (scohg : SizedCospanHyperGraph N T n m) :
+  SizedCospanHyperGraph N T n m :=
+  mk_scohg (relabel_graph {[k := k']} scohg) (map_relabel_one k' k scohg.(sized_map)).
+
+
+Definition relabels_sized_graph_r {n m} {l} (ks : vec (positive * positive) l)
+  (scohg : SizedCospanHyperGraph N T n m) : SizedCospanHyperGraph N T n m :=
+  mk_scohg (relabel_graph (subst_by_vec (propogate_subst ks)) scohg)
+    (map_relabels_r ks (scohg.(sized_map))).
+
+Lemma sized_add_top_loop_eq_relabel_one {n m} (scohg : SizedCospanHyperGraph N T (S n) (S m)) :
+  sized_add_top_loop scohg =
+  sized_add_top_loop (relabel_sized_graph_one (vhd (outputs scohg)) (vhd (inputs scohg)) scohg).
+Proof.
+  apply scohg_ext; [apply add_top_loop_eq_relabel|].
+  cbn.
+  rewrite 2 vhd_vmap.
+  rewrite fn_lookup_singleton, fn_lookup_singleton_r.
+  apply map_eq.
+  intros i.
+  rewrite 3 lookup_map_relabel_one.
+  rewrite fn_lookup_singleton_id.
+  done.
+Qed.
+
+Lemma sized_add_top_loop_struct_sized_isomorphic_strong {n m} (scohg scohg' : SizedCospanHyperGraph N T (S n) (S m)) :
+  relabel_sized_graph_one (vhd (outputs scohg)) (vhd (inputs scohg)) scohg ≡ᵢ
+  relabel_sized_graph_one (vhd (outputs scohg')) (vhd (inputs scohg')) scohg' ->
+  sized_add_top_loop scohg ≡ᵢ sized_add_top_loop scohg'.
+Proof.
+  intros Hiso.
+  rewrite sized_add_top_loop_eq_relabel_one.
+  erewrite sized_add_top_loop_struct_sized_isomorphic by apply Hiso.
+  rewrite <- sized_add_top_loop_eq_relabel_one.
+  done.
+Qed.
+
+
+
+
+Lemma sized_add_top_loops_struct_sized_isomorphic {n m o}
+  (scohg scohg' : SizedCospanHyperGraph N T (n + m) (n + o)) :
+  scohg ≡ᵢ scohg' ->
+  sized_add_top_loops scohg ≡ᵢ sized_add_top_loops scohg'.
+Proof.
+  intros Hiso.
+  induction n; [done|].
+  cbn.
+  apply IHn.
+  now apply sized_add_top_loop_struct_sized_isomorphic.
+Qed.
+
+Lemma compose_sized_graphs_struct_sized_isomorphic {n m o}
+  (scohg1 scohg1' : SizedCospanHyperGraph N T n m) (scohg2 scohg2' : SizedCospanHyperGraph N T m o) :
+  scohg1 ≡ᵢ scohg1' -> scohg2 ≡ᵢ scohg2' ->
+  compose_sized_graphs scohg1 scohg2 ≡ᵢ compose_sized_graphs scohg1' scohg2'.
+Proof.
+  intros Heq1 Heq2.
+  rewrite <- 2 compose_sized_graphs_alt_correct.
+  apply sized_add_top_loops_struct_sized_isomorphic.
+  now apply swapped_stack_sized_graphs_struct_sized_isomorphic.
+Qed.
+
+
+
+
+
+#[export] Instance sized_add_top_loops_scohg_vert_eq {n m o} :
+  Proper (scohg_vert_eq ==> scohg_vert_eq)
+    (@sized_add_top_loops N T n m o).
+Proof.
+  induction n; [easy|].
+  intros scohg scohg' Hscohg.
+  cbn.
+  now apply IHn, sized_add_top_loop_proper.
+Qed.
+
+
+
+#[export] Instance compose_sized_graphs_alt_scohg_vert_eq
+  {n m o} : Proper (scohg_vert_eq ==> scohg_vert_eq ==> scohg_vert_eq)
+    (@compose_sized_graphs_alt N T n m o).
+Proof.
+  intros scohg1 scohg1' Hscohg1 scohg2 scohg2' Hscohg2.
+  unfold compose_sized_graphs_alt.
+  now do 2 f_equiv.
+Qed.
+
+#[export] Instance compose_sized_graphs_alt_struct_sized_isomorphic `{Equiv T, Equivalence T equiv}
+  {n m o} : Proper (struct_sized_isomorphic ==> struct_sized_isomorphic ==> struct_sized_isomorphic)
+    (@compose_sized_graphs_alt N T n m o).
+Proof.
+  intros scohg1 scohg1' Hscohg1 scohg2 scohg2' Hscohg2.
+  unfold compose_sized_graphs_alt.
+  apply sized_add_top_loops_struct_sized_isomorphic.
+  now apply swapped_stack_sized_graphs_struct_sized_isomorphic.
+Qed.
+
+(* FIXME: Move *)
+#[export] Instance struct_sized_isomorphic_syntactic_eq {T'} `{Equiv T', Equivalence T' equiv} {n m} :
+  subrelation (@struct_sized_isomorphic N T' n m) scohg_syntactic_eq.
+Proof.
+  intros x y Heq.
+  hnf in Heq.
+  rewrite <- (norm_sized_verts_vert_eq x), Heq.
+  apply (subrel (norm_sized_verts_vert_eq y)).
+Qed.
+
+(*
+#[export] Instance scohg_vert_eq_struct_sized_isomorphic {n m} :
+  subrelation (@scohg_vert_eq N T n m) struct_sized_isomorphic.
+  apply _.
+Proof.
+  now intros ? ? <-.
+Qed. *)
+
+
+Lemma proper_scohg_syntactic_eq_of_struct_sized_iso_eq_binary `{Equiv T1, Equivalence T1 equiv,
+  Equiv T2, Equivalence T2 equiv, Equiv T3, Equivalence T3 equiv} {n1 m1 n2 m2 n3 m3}
+  (f : SizedCospanHyperGraph N T1 n1 m1 -> SizedCospanHyperGraph N T2 n2 m2 ->
+    SizedCospanHyperGraph N T3 n3 m3) :
+  Proper (struct_sized_isomorphic ==> struct_sized_isomorphic ==> struct_sized_isomorphic) f ->
+  Proper (scohg_eq ==> scohg_eq ==> scohg_eq) f ->
+  Proper (scohg_syntactic_eq ==> scohg_syntactic_eq ==> scohg_syntactic_eq) f.
+Proof.
+  intros Hfiso Hfscohg.
+  intros scohg1 scohg1' Hscohg1 scohg2 scohg2' Hscohg2.
+  induction Hscohg1 as [scohg1 scohg1' fv1 fe1 Hfv1 Hfe1 Hverteq1].
+  rewrite <- (subrel'' struct_sized_isomorphic (norm_sized_verts_vert_eq scohg1)).
+  rewrite (Hverteq1).
+  rewrite (subrel'' struct_sized_isomorphic (norm_sized_verts_vert_eq _)).
+  rewrite <- (subrel'' struct_sized_isomorphic (sized_iso_relabel_reindex _ _ _)) by done.
+  induction Hscohg2 as [scohg2 scohg2' fv2 fe2 Hfv2 Hfe2 Hverteq2].
+  rewrite <- (subrel'' struct_sized_isomorphic (norm_sized_verts_vert_eq scohg2)).
+  rewrite (Hverteq2).
+  rewrite (subrel'' struct_sized_isomorphic (norm_sized_verts_vert_eq _)).
+  rewrite <- (subrel'' struct_sized_isomorphic (sized_iso_relabel_reindex _ _ _)) by done.
+  done.
+Qed.
+
+#[export] Instance compose_sized_graphs_alt_scohg_syntactic_eq `{Equiv T, Equivalence T equiv}
+  {n m o} : Proper (scohg_syntactic_eq ==> scohg_syntactic_eq ==> scohg_syntactic_eq)
+    (@compose_sized_graphs_alt N T n m o).
+Proof.
+  apply proper_scohg_syntactic_eq_of_struct_sized_iso_eq_binary; apply _.
+Qed.
+
+#[export] Instance compose_sized_graphs_scohg_vert_eq
+  {n m o} : Proper (scohg_vert_eq ==> scohg_vert_eq ==> scohg_vert_eq)
+    (@compose_sized_graphs N T n m o).
+Proof.
+  intros scohg1 scohg1' Hscohg1 scohg2 scohg2' Hscohg2.
+  do 2 rewrite <- compose_sized_graphs_alt_correct.
+  now do 2 f_equiv.
+Qed.
+
+#[export] Instance compose_sized_graphs_struct_sized_isomorphic_mor `{Equiv T, Equivalence T equiv}
+  {n m o} : Proper (struct_sized_isomorphic ==> struct_sized_isomorphic ==> struct_sized_isomorphic)
+    (@compose_sized_graphs N T n m o).
+Proof.
+  intros scohg1 scohg1' Hscohg1 scohg2 scohg2' Hscohg2.
+  do 2 rewrite <- compose_sized_graphs_alt_correct.
+  now apply compose_sized_graphs_alt_struct_sized_isomorphic.
+Qed.
+
+#[export] Instance compose_sized_graphs_scohg_syntactic_eq `{Equiv T, Equivalence T equiv}
+  {n m o} : Proper (scohg_syntactic_eq ==> scohg_syntactic_eq ==> scohg_syntactic_eq)
+    (@compose_sized_graphs N T n m o).
+Proof.
+  intros scohg1 scohg1' Hscohg1 scohg2 scohg2' Hscohg2.
+  rewrite <- 2 compose_sized_graphs_alt_correct.
+  now apply compose_sized_graphs_alt_scohg_syntactic_eq.
+Qed.
+
+#[export] Instance stack_sized_graphs_scohg_syntactic_eq `{Equiv T, Equivalence T equiv}
+  {n m o p} : Proper (scohg_syntactic_eq ==> scohg_syntactic_eq ==> scohg_syntactic_eq)
+    (@stack_sized_graphs N T n m o p).
+Proof.
+  apply proper_scohg_syntactic_eq_of_struct_sized_iso_eq_binary; apply _.
+Qed.
+
+#[export] Instance compose_sized_graphs_aux_scohg_eq `{Equiv T} {n m o} :
+  Proper (scohg_eq ==> scohg_eq ==> scohg_eq) (@compose_sized_graphs_aux N T n m o).
+Proof.
+  intros cohg1 cohg1' Heq1 cohg2 cohg2' Heq2.
+  split; [apply compose_graphs_aux_cohg_eq, Heq2.1; apply Heq1.1|].
+  cbn.
+  f_equal; (f_equal; [apply Heq1|apply Heq2]).
+Qed.
+
+
+#[export] Instance compose_sized_graphs_scohg_eq `{Equiv T} {n m o} :
+  Proper (scohg_eq ==> scohg_eq ==> scohg_eq) (@compose_sized_graphs N T n m o).
+Proof.
+  intros scohg1 scohg1' Hscohg1 scohg2 scohg2' Hscohg2.
+  rewrite 2 compose_sized_graphs_to_compose_sized_graphs_aux.
+  now apply compose_sized_graphs_aux_scohg_eq; do 2 f_equiv.
+Qed.
+
+
+
+
+
+
+
+
+
+
+
+
+(* 
+
+
+
+
+
+
+
+
+
+
+Lemma sized_add_top_loops_eq_relabels {n m m'}
+  (scohg : SizedCospanHyperGraph N T (n + m) (n + m')) :
+  sized_add_top_loops scohg =
+  sized_add_top_loops (relabels_sized_graph_r
+    (vzip (vsplitl (outputs scohg)) (vsplitl (inputs scohg))) scohg).
+Proof.
+  apply scohg_ext; [
+    rewrite 2 sized_cospan_sized_add_top_loops; apply add_top_loops_eq_relabel|].
+  rewrite 2 sized_map_sized_add_top_loops.
+  cbn.
+  destruct scohg as [[hg ins outs] smap].
+  cbn.
+  induction ins as [lins rins] using vec_add_inv.
+  induction outs as [louts routs] using vec_add_inv.
+  rewrite 2 vsplitl_app, 2 vsplitl_map, 2 vsplitl_app.
+  clear.
+
+
+  unfold sized_add_top_loops.
+  induction n; [cbn; now rewrite relabel_sized_graph_id|].
+  cbn -[propogate_subst].
+  rewrite IHn.
+  f_equal.
+  destruct scohg as [hg ins outs].
+  induction ins as [insl insr] using vec_add_inv.
+  induction outs as [outsl outsr] using vec_add_inv.
+  induction insl as [i insl] using vec_S_inv.
+  induction outsl as [o outsl] using vec_S_inv.
+  cbn -[propogate_subst Vector.append].
+  rewrite 2 vsplitl_app.
+  cbn -[propogate_subst].
+  rewrite 2 vsplitl_map, 2 vsplitl_app.
+  apply scohg_ext.
+  - cbn.
+    rewrite relabel_hg_compose, 2 relabel_hg_add_vertices, relabel_hg_compose.
+    f_equal. 2:{
+      rewrite 2 set_map_singleton_L.
+      rewrite fn_lookup_singleton_r.
+      cbn.
+      rewrite vzip_map.
+      done.
+    }
+    apply relabel_hg_ext.
+    intros k.
+    cbn.
+    rewrite fn_lookup_singleton, fn_lookup_singleton_r.
+    rewrite fn_lookup_singleton_id.
+    rewrite vzip_map.
+    done.
+  - cbn -[Vector.append propogate_subst].
+    rewrite 2 Vector.map_map.
+    apply Vector.map_ext.
+    intros k.
+    rewrite vzip_map.
+    cbn.
+    rewrite fn_lookup_singleton, fn_lookup_singleton_r.
+    rewrite fn_lookup_singleton_id.
+    done.
+  - cbn -[Vector.append propogate_subst].
+    rewrite 2 Vector.map_map.
+    apply Vector.map_ext.
+    intros k.
+    rewrite vzip_map.
+    cbn.
+    rewrite fn_lookup_singleton, fn_lookup_singleton_r.
+    rewrite fn_lookup_singleton_id.
+    done.
+Qed.
+
+
+Lemma sized_add_top_loops_eq_relabel {n m m'}
+  (scohg : SizedCospanHyperGraph N T (n + m) (n + m')) :
+  sized_add_top_loops scohg =
+  sized_add_top_loops (relabel_sized_graph (subst_by_vec (propogate_subst
+    $ vzip (vsplitl (outputs scohg)) (vsplitl (inputs scohg)))) scohg).
+Proof.
+  induction n; [cbn; now rewrite relabel_sized_graph_id|].
+  cbn -[propogate_subst].
+  rewrite IHn.
+  f_equal.
+  destruct scohg as [hg ins outs].
+  induction ins as [insl insr] using vec_add_inv.
+  induction outs as [outsl outsr] using vec_add_inv.
+  induction insl as [i insl] using vec_S_inv.
+  induction outsl as [o outsl] using vec_S_inv.
+  cbn -[propogate_subst Vector.append].
+  rewrite 2 vsplitl_app.
+  cbn -[propogate_subst].
+  rewrite 2 vsplitl_map, 2 vsplitl_app.
+  apply scohg_ext.
+  - cbn.
+    rewrite relabel_hg_compose, 2 relabel_hg_add_vertices, relabel_hg_compose.
+    f_equal. 2:{
+      rewrite 2 set_map_singleton_L.
+      rewrite fn_lookup_singleton_r.
+      cbn.
+      rewrite vzip_map.
+      done.
+    }
+    apply relabel_hg_ext.
+    intros k.
+    cbn.
+    rewrite fn_lookup_singleton, fn_lookup_singleton_r.
+    rewrite fn_lookup_singleton_id.
+    rewrite vzip_map.
+    done.
+  - cbn -[Vector.append propogate_subst].
+    rewrite 2 Vector.map_map.
+    apply Vector.map_ext.
+    intros k.
+    rewrite vzip_map.
+    cbn.
+    rewrite fn_lookup_singleton, fn_lookup_singleton_r.
+    rewrite fn_lookup_singleton_id.
+    done.
+  - cbn -[Vector.append propogate_subst].
+    rewrite 2 Vector.map_map.
+    apply Vector.map_ext.
+    intros k.
+    rewrite vzip_map.
+    cbn.
+    rewrite fn_lookup_singleton, fn_lookup_singleton_r.
+    rewrite fn_lookup_singleton_id.
+    done.
+Qed.
+
+Lemma sized_add_top_loops_struct_sized_isomorphic_strong {n m o}
+  (scohg scohg' : SizedCospanHyperGraph N T (n + m) (n + o)) :
+  relabel_sized_graph (subst_by_vec (propogate_subst
+    $ vzip (vsplitl (outputs scohg)) (vsplitl (inputs scohg)))) scohg ≡ᵢ
+  relabel_sized_graph (subst_by_vec (propogate_subst
+    $ vzip (vsplitl (outputs scohg')) (vsplitl (inputs scohg')))) scohg' ->
+  sized_add_top_loops scohg ≡ᵢ sized_add_top_loops scohg'.
+Proof.
+  intros Hiso.
+  rewrite sized_add_top_loops_eq_relabel.
+  erewrite sized_add_top_loops_struct_sized_isomorphic by apply Hiso.
+  rewrite <- sized_add_top_loops_eq_relabel.
+  done.
+Qed.
+
+
+
+
+Lemma relabel_sized_graph_to_fun_to_map {n m} f (scohg : SizedCospanHyperGraph N T n m) :
+  relabel_sized_graph f scohg = relabel_sized_graph (Pmap_map (fun_to_map f (vertices scohg))) scohg.
+Proof.
+  apply relabel_sized_graph_ext_strong.
+  intros i Hi.
+  symmetry.
+  unfold Pmap_map.
+  now rewrite lookup_fun_to_map_Some_1.
+Qed.
+
+Lemma relabel_sized_graph_Pmap_map_to_union_l {n m} ml mr (scohg : SizedCospanHyperGraph N T n m) :
+  vertices scohg ⊆ dom ml ->
+  relabel_sized_graph (Pmap_map ml) scohg =
+  relabel_sized_graph (Pmap_map (ml ∪ mr)) scohg.
+Proof.
+  intros Hvert.
+  apply relabel_sized_graph_ext_strong.
+  intros i [mli Hmli]%Hvert%elem_of_dom.
+  unfold Pmap_map.
+  rewrite lookup_union, Hmli.
+  now destruct (mr !! i).
+Qed.
+
+Lemma relabel_sized_graph_Pmap_map_to_union_r {n m} ml mr (scohg : SizedCospanHyperGraph N T n m) :
+  vertices scohg ## dom ml ->
+  relabel_sized_graph (Pmap_map mr) scohg =
+  relabel_sized_graph (Pmap_map (ml ∪ mr)) scohg.
+Proof.
+  intros Hvert.
+  apply relabel_sized_graph_ext_strong.
+  intros i Hi%Hvert%not_elem_of_dom.
+  unfold Pmap_map.
+  rewrite lookup_union, Hi.
+  now rewrite (left_id_L None _).
+Qed.
+
+Lemma relabel_sized_graph_Pmap_map_to_Pmap_injmap {n m} mv (scohg : SizedCospanHyperGraph N T n m) :
+  vertices scohg ⊆ dom mv ->
+  relabel_sized_graph (Pmap_map mv) scohg =
+  relabel_sized_graph (Pmap_injmap mv) scohg.
+Proof.
+  intros Hvert.
+  apply relabel_sized_graph_ext_strong.
+  intros i Hi%Hvert.
+  symmetry.
+  now apply Pmap_injmap_correct_dom.
+Qed.
+
+Lemma reindex_sized_graph_to_fun_to_map {n m} f (scohg : SizedCospanHyperGraph N T n m) :
+  reindex_sized_graph f scohg = reindex_sized_graph (Pmap_map (fun_to_map f (dom (hyperedges scohg)))) scohg.
+Proof.
+  apply reindex_sized_graph_ext_strong.
+  intros i _ Hi%elem_of_dom_2.
+  symmetry.
+  unfold Pmap_map.
+  now rewrite lookup_fun_to_map_Some_1.
+Qed.
+
+Lemma reindex_sized_graph_Pmap_map_to_union_l {n m} ml mr (scohg : SizedCospanHyperGraph N T n m) :
+  dom $ hyperedges scohg ⊆ dom ml ->
+  reindex_sized_graph (Pmap_map ml) scohg =
+  reindex_sized_graph (Pmap_map (ml ∪ mr)) scohg.
+Proof.
+  intros Hvert.
+  apply reindex_sized_graph_ext_strong.
+  intros i _ [mli Hmli]%elem_of_dom_2%Hvert%elem_of_dom.
+  unfold Pmap_map.
+  rewrite lookup_union, Hmli.
+  now destruct (mr !! i).
+Qed.
+
+Lemma reindex_sized_graph_Pmap_map_to_union_r {n m} ml mr (scohg : SizedCospanHyperGraph N T n m) :
+  dom $ hyperedges scohg ## dom ml ->
+  reindex_sized_graph (Pmap_map mr) scohg =
+  reindex_sized_graph (Pmap_map (ml ∪ mr)) scohg.
+Proof.
+  intros Hvert.
+  apply reindex_sized_graph_ext_strong.
+  intros i _ Hi%elem_of_dom_2%Hvert%not_elem_of_dom.
+  unfold Pmap_map.
+  rewrite lookup_union, Hi.
+  now rewrite (left_id_L None _).
+Qed.
+
+Lemma reindex_sized_graph_Pmap_map_to_Pmap_injmap {n m} mv (scohg : SizedCospanHyperGraph N T n m) :
+  dom $ hyperedges scohg ⊆ dom mv ->
+  reindex_sized_graph (Pmap_map mv) scohg =
+  reindex_sized_graph (Pmap_injmap mv) scohg.
+Proof.
+  intros Hvert.
+  apply reindex_sized_graph_ext_strong.
+  intros i _ Hi%elem_of_dom_2%Hvert.
+  symmetry.
+  now apply Pmap_injmap_correct_dom.
+Qed.
+
+(* FIXME: Move *)
+Lemma map_inj_disj_union `{FinMap K M} {A}
+  (m1 m2 : M A) :
+  m1 ##ₘ m2 ->
+  map_inj m1 -> map_inj m2 ->
+  (forall i j a b, m1 !! i = Some a -> m2 !! j = Some b -> a <> b) ->
+  map_inj (m1 ∪ m2).
+Proof.
+  intros Hdisj Hinj1 Hinj2 Hdisjimg.
+  intros i j a.
+  rewrite 2 lookup_union_Some by done.
+  intros [Hm1i|Hm2i] [Hm1j|Hm2j]; [now eauto|..|now eauto];
+  exfalso; eapply (Hdisjimg _ _ a); eauto.
+Qed.
+Lemma fun_to_map_inj `{FinMap K M, FinSet K SK} {A}
+  (f : K -> A) `{Hf : !Inj eq eq f} (X : SK) :
+  map_inj (fun_to_map f X :> M A).
+Proof.
+  intros i j a.
+  rewrite 2 lookup_fun_to_map_Some.
+  now intros [Hi <-] [Hj ?%Hf].
+Qed.
+Lemma map_img_fun_to_map `{FinMap K M, FinSet K SK, SemiSet A SA}
+  (f : K -> A) (X : SK) :
+  map_img (fun_to_map f X :> M A) ≡@{SA} set_map f X.
+Proof.
+  intros k.
+  rewrite elem_of_map, elem_of_map_img.
+  setoid_rewrite lookup_fun_to_map_Some.
+  firstorder.
+Qed.
+Lemma map_img_fun_to_map_L `{FinMap K M, FinSet K SK, SemiSet A SA, !LeibnizEquiv SA}
+  (f : K -> A) (X : SK) :
+  map_img (fun_to_map f X :> M A) =@{SA} set_map f X.
+Proof.
+  apply leibniz_equiv_iff, map_img_fun_to_map.
+Qed.
+
+
+Lemma stack_sized_graphs_aux_relabel_disjoint {n m n' m'} f1 f2
+  (scohg1 : SizedCospanHyperGraph N T n m) (scohg2 : SizedCospanHyperGraph N T n' m') :
+  vertices scohg1 ## vertices scohg2 ->
+  stack_sized_graphs_aux (relabel_sized_graph f1 scohg1) (relabel_sized_graph f2 scohg2) =
+  relabel_sized_graph (Pmap_map (fun_to_map f1 (vertices scohg1) ∪ fun_to_map f2 (vertices scohg2)))
+    (stack_sized_graphs_aux scohg1 scohg2).
+Proof.
+  intros Hdisj.
+  rewrite relabel_stack_sized_graphs_aux.
+  f_equal.
+  - rewrite (relabel_sized_graph_to_fun_to_map f1).
+    apply relabel_sized_graph_Pmap_map_to_union_l.
+    now rewrite dom_fun_to_map_L.
+  - rewrite (relabel_sized_graph_to_fun_to_map f2).
+    apply relabel_sized_graph_Pmap_map_to_union_r.
+    now rewrite dom_fun_to_map_L.
+Qed.
+
+Lemma stack_sized_graphs_aux_reindex_disjoint {n m n' m'} f1 f2
+  `{Hf1 : !Inj eq eq f1, Hf2 : !Inj eq eq f2}
+  (scohg1 : SizedCospanHyperGraph N T n m) (scohg2 : SizedCospanHyperGraph N T n' m') :
+  dom $ hyperedges scohg1 ## dom $ hyperedges scohg2 ->
+  set_map f1 $ dom $ hyperedges scohg1 ##@{Pset} set_map f2 $ dom $ hyperedges scohg2 ->
+  stack_sized_graphs_aux (reindex_sized_graph f1 scohg1) (reindex_sized_graph f2 scohg2) =
+  reindex_sized_graph (Pmap_map (fun_to_map f1 (dom $ hyperedges scohg1) ∪
+    fun_to_map f2 (dom $ hyperedges scohg2)))
+    (stack_sized_graphs_aux scohg1 scohg2).
+Proof.
+  intros Hdisj Hdisjran.
+  rewrite reindex_sized_graph_Pmap_map_to_Pmap_injmap. 2:{
+    cbn.
+    rewrite 2 dom_union_L, 2 dom_fun_to_map_L.
+    done.
+  }
+  rewrite reindex_stack_sized_graphs_aux; [f_equal|].
+  - rewrite (reindex_sized_graph_to_fun_to_map f1).
+    rewrite <- reindex_sized_graph_Pmap_map_to_Pmap_injmap by
+      now rewrite dom_union_L, 2 dom_fun_to_map_L, <- union_subseteq_l'.
+    apply reindex_sized_graph_Pmap_map_to_union_l.
+    now rewrite dom_fun_to_map_L.
+  - rewrite (reindex_sized_graph_to_fun_to_map f2).
+    rewrite <- reindex_sized_graph_Pmap_map_to_Pmap_injmap by
+      now rewrite dom_union_L, 2 dom_fun_to_map_L, <- union_subseteq_r'.
+    apply reindex_sized_graph_Pmap_map_to_union_r.
+    now rewrite dom_fun_to_map_L.
+  - apply Pmap_injmap_inj.
+    apply map_inj_disj_union.
+    + now rewrite map_disjoint_dom, 2 dom_fun_to_map_L.
+    + now apply fun_to_map_inj.
+    + now apply fun_to_map_inj.
+    + intros i j a b Ha%(elem_of_map_img_2 (SA:=Pset))
+        Hb%(elem_of_map_img_2 (SA:=Pset)).
+      rewrite map_img_fun_to_map_L in Ha, Hb.
+      intros ->.
+      apply Hdisjran in Ha.
+      now apply Ha in Hb.
+Qed.
+
+
+Lemma stack_sized_graphs_aux_sized_isomorphic {n m n' m'}
+  (scohg1 scohg1' : SizedCospanHyperGraph N T n m)
+  (scohg2 scohg2' : SizedCospanHyperGraph N T n' m') :
+  sized_isomorphic scohg1 scohg1' -> sized_isomorphic scohg2 scohg2' ->
+  hyperedges scohg1 ##ₘ hyperedges scohg2 -> hyperedges scohg1' ##ₘ hyperedges scohg2' ->
+  vertices scohg1 ## vertices scohg2 -> vertices scohg1' ## vertices scohg2' ->
+  sized_isomorphic (stack_sized_graphs_aux scohg1 scohg2) (stack_sized_graphs_aux scohg1' scohg2').
+Proof.
+  intros (fv1 & fe1 & Hfv1 & Hfe1 & ->)%sized_isomorphic_exists
+    (fv2 & fe2 & Hfv2 & Hfe2 & ->)%sized_isomorphic_exists.
+  intros Hdisj Hdisj' Hvdisj Hvdisj'.
+  rewrite stack_sized_graphs_aux_relabel_disjoint by now rewrite 2 (vertices_reindex_sized_graph _).
+  rewrite (stack_sized_graphs_aux_reindex_disjoint _ _ _); [|now apply map_disjoint_dom|].
+  2:{
+    rewrite map_disjoint_dom in Hdisj'.
+    cbn in Hdisj'.
+    rewrite 2 dom_fmap_L in Hdisj'.
+    rewrite 2 dom_kmap_L' in Hdisj'.
+    done.
+  }
+  rewrite reindex_sized_graph_Pmap_map_to_Pmap_injmap. 2:{
+    cbn.
+    now rewrite 2 dom_union_L, 2 dom_fun_to_map_L.
+  }
+  assert (Hinjidx : Inj eq eq (Pmap_injmap
+           (fun_to_map fe1 (dom (hyperedges scohg1) :> Pset) ∪
+           fun_to_map fe2 (dom (hyperedges scohg2) :> Pset)))). 1:{
+    apply Pmap_injmap_inj.
+    apply map_inj_disj_union.
+    + now rewrite map_disjoint_dom, 2 dom_fun_to_map_L; rewrite map_disjoint_dom in Hdisj.
+    + now apply fun_to_map_inj.
+    + now apply fun_to_map_inj.
+    + intros i j a b Ha%(elem_of_map_img_2 (SA:=Pset))
+        Hb%(elem_of_map_img_2 (SA:=Pset)).
+      rewrite map_img_fun_to_map_L in Ha, Hb.
+      rewrite map_disjoint_dom in Hdisj'.
+      cbn in Hdisj'.
+      rewrite 2 dom_fmap, 2 dom_kmap_L' in Hdisj'.
+      intros ->.
+      now apply Hdisj' in Hb.
+  }
+  rewrite relabel_sized_graph_Pmap_map_to_Pmap_injmap. 2:{
+    rewrite 3 (vertices_reindex_sized_graph _).
+    rewrite vertices_stack_sized_graphs_aux by done.
+    now rewrite dom_union_L, 2 dom_fun_to_map_L.
+  }
+  constructor.
+  - apply Pmap_injmap_inj.
+    apply map_inj_disj_union.
+    + now rewrite map_disjoint_dom, 2 dom_fun_to_map_L,
+      2 (vertices_reindex_sized_graph _).
+    + now apply fun_to_map_inj.
+    + now apply fun_to_map_inj.
+    + intros i j a b Ha%(elem_of_map_img_2 (SA:=Pset))
+        Hb%(elem_of_map_img_2 (SA:=Pset)).
+      rewrite map_img_fun_to_map_L in Ha, Hb.
+      rewrite (vertices_reindex_sized_graph _) in Ha.
+      rewrite (vertices_reindex_sized_graph _) in Hb.
+      rewrite 2 vertices_relabel_sized_graph, 2 (vertices_reindex_sized_graph _) in Hvdisj'.
+      intros ->.
+      now apply Hvdisj' in Hb.
+  - apply _.
+Qed.
+
+
+Lemma stack_sized_graphs_aux_to_stack_sized_graphs_disjoint {n m n' m'}
+  (scohg1 : SizedCospanHyperGraph N T n m) (scohg2 : SizedCospanHyperGraph N T n' m') :
+  hyperedges scohg1 ##ₘ hyperedges scohg2 ->
+  vertices scohg1 ## vertices scohg2 ->
+  sized_isomorphic (stack_sized_graphs_aux scohg1 scohg2) (stack_sized_graphs scohg1 scohg2).
+Proof.
+  intros Hdisj Hvdisj.
+  unfold stack_sized_graphs.
+  apply stack_sized_graphs_aux_sized_isomorphic.
+  - constructor; apply _.
+  - constructor; apply _.
+  - done.
+  - cbn.
+    apply map_disjoint_fmap.
+    now apply (kmap_inj2_disjoint _).
+  - done.
+  - rewrite 2 vertices_relabel_sized_graph, 2 (vertices_reindex_sized_graph _).
+    set_solver +.
+Qed.
+
+
+Lemma swapped_stack_sized_graphs_aux_relabel_disjoint {n m n' m'} f1 f2
+  (scohg1 : SizedCospanHyperGraph N T n m) (scohg2 : SizedCospanHyperGraph N T n' m') :
+  vertices scohg1 ## vertices scohg2 ->
+  swapped_stack_sized_graphs_aux (relabel_sized_graph f1 scohg1) (relabel_sized_graph f2 scohg2) =
+  relabel_sized_graph (Pmap_map (fun_to_map f1 (vertices scohg1) ∪ fun_to_map f2 (vertices scohg2)))
+    (swapped_stack_sized_graphs_aux scohg1 scohg2).
+Proof.
+  intros Hdisj.
+  rewrite relabel_swapped_stack_sized_graphs_aux.
+  f_equal.
+  - rewrite (relabel_sized_graph_to_fun_to_map f1).
+    apply relabel_sized_graph_Pmap_map_to_union_l.
+    now rewrite dom_fun_to_map_L.
+  - rewrite (relabel_sized_graph_to_fun_to_map f2).
+    apply relabel_sized_graph_Pmap_map_to_union_r.
+    now rewrite dom_fun_to_map_L.
+Qed.
+
+Lemma swapped_stack_sized_graphs_aux_reindex_disjoint {n m n' m'} f1 f2
+  `{Hf1 : !Inj eq eq f1, Hf2 : !Inj eq eq f2}
+  (scohg1 : SizedCospanHyperGraph N T n m) (scohg2 : SizedCospanHyperGraph N T n' m') :
+  dom $ hyperedges scohg1 ## dom $ hyperedges scohg2 ->
+  set_map f1 $ dom $ hyperedges scohg1 ##@{Pset} set_map f2 $ dom $ hyperedges scohg2 ->
+  swapped_stack_sized_graphs_aux (reindex_sized_graph f1 scohg1) (reindex_sized_graph f2 scohg2) =
+  reindex_sized_graph (Pmap_map (fun_to_map f1 (dom $ hyperedges scohg1) ∪
+    fun_to_map f2 (dom $ hyperedges scohg2)))
+    (swapped_stack_sized_graphs_aux scohg1 scohg2).
+Proof.
+  intros Hdisj Hdisjran.
+  rewrite reindex_sized_graph_Pmap_map_to_Pmap_injmap. 2:{
+    cbn.
+    rewrite 2 dom_union_L, 2 dom_fun_to_map_L.
+    done.
+  }
+  rewrite reindex_swapped_stack_sized_graphs_aux; [f_equal|].
+  - rewrite (reindex_sized_graph_to_fun_to_map f1).
+    rewrite <- reindex_sized_graph_Pmap_map_to_Pmap_injmap by
+      now rewrite dom_union_L, 2 dom_fun_to_map_L, <- union_subseteq_l'.
+    apply reindex_sized_graph_Pmap_map_to_union_l.
+    now rewrite dom_fun_to_map_L.
+  - rewrite (reindex_sized_graph_to_fun_to_map f2).
+    rewrite <- reindex_sized_graph_Pmap_map_to_Pmap_injmap by
+      now rewrite dom_union_L, 2 dom_fun_to_map_L, <- union_subseteq_r'.
+    apply reindex_sized_graph_Pmap_map_to_union_r.
+    now rewrite dom_fun_to_map_L.
+  - apply Pmap_injmap_inj.
+    apply map_inj_disj_union.
+    + now rewrite map_disjoint_dom, 2 dom_fun_to_map_L.
+    + now apply fun_to_map_inj.
+    + now apply fun_to_map_inj.
+    + intros i j a b Ha%(elem_of_map_img_2 (SA:=Pset))
+        Hb%(elem_of_map_img_2 (SA:=Pset)).
+      rewrite map_img_fun_to_map_L in Ha, Hb.
+      intros ->.
+      apply Hdisjran in Ha.
+      now apply Ha in Hb.
+Qed.
+
+Lemma vertices_swapped_stack_sized_graphs_aux {n m n' m'}
+  (scohg1 : SizedCospanHyperGraph N T n m) (scohg2 : SizedCospanHyperGraph N T n' m') :
+  hyperedges scohg1 ##ₘ hyperedges scohg2 ->
+  vertices (swapped_stack_sized_graphs_aux scohg1 scohg2) =
+  vertices scohg1 ∪ vertices scohg2.
+Proof.
+  intros Hdisj.
+  unfold vertices.
+  cbn.
+  rewrite vertices_hg_union by done.
+  rewrite 2 vec_to_list_app, 5 list_to_set_app_L.
+  apply set_eq.
+  intros k.
+  rewrite !elem_of_union.
+  tauto.
+Qed.
+
+Lemma swapped_stack_sized_graphs_aux_sized_isomorphic {n m n' m'}
+  (scohg1 scohg1' : SizedCospanHyperGraph N T n m)
+  (scohg2 scohg2' : SizedCospanHyperGraph N T n' m') :
+  sized_isomorphic scohg1 scohg1' -> sized_isomorphic scohg2 scohg2' ->
+  hyperedges scohg1 ##ₘ hyperedges scohg2 -> hyperedges scohg1' ##ₘ hyperedges scohg2' ->
+  vertices scohg1 ## vertices scohg2 -> vertices scohg1' ## vertices scohg2' ->
+  sized_isomorphic (swapped_stack_sized_graphs_aux scohg1 scohg2) (swapped_stack_sized_graphs_aux scohg1' scohg2').
+Proof.
+  intros (fv1 & fe1 & Hfv1 & Hfe1 & ->)%sized_isomorphic_exists
+    (fv2 & fe2 & Hfv2 & Hfe2 & ->)%sized_isomorphic_exists.
+  intros Hdisj Hdisj' Hvdisj Hvdisj'.
+  rewrite swapped_stack_sized_graphs_aux_relabel_disjoint by now rewrite 2 (vertices_reindex_sized_graph _).
+  rewrite (swapped_stack_sized_graphs_aux_reindex_disjoint _ _ _); [|now apply map_disjoint_dom|].
+  2:{
+    rewrite map_disjoint_dom in Hdisj'.
+    cbn in Hdisj'.
+    rewrite 2 dom_fmap_L in Hdisj'.
+    rewrite 2 dom_kmap_L' in Hdisj'.
+    done.
+  }
+  rewrite reindex_sized_graph_Pmap_map_to_Pmap_injmap. 2:{
+    cbn.
+    now rewrite 2 dom_union_L, 2 dom_fun_to_map_L.
+  }
+  assert (Hinjidx : Inj eq eq (Pmap_injmap
+           (fun_to_map fe1 (dom (hyperedges scohg1) :> Pset) ∪
+           fun_to_map fe2 (dom (hyperedges scohg2) :> Pset)))). 1:{
+    apply Pmap_injmap_inj.
+    apply map_inj_disj_union.
+    + now rewrite map_disjoint_dom, 2 dom_fun_to_map_L; rewrite map_disjoint_dom in Hdisj.
+    + now apply fun_to_map_inj.
+    + now apply fun_to_map_inj.
+    + intros i j a b Ha%(elem_of_map_img_2 (SA:=Pset))
+        Hb%(elem_of_map_img_2 (SA:=Pset)).
+      rewrite map_img_fun_to_map_L in Ha, Hb.
+      rewrite map_disjoint_dom in Hdisj'.
+      cbn in Hdisj'.
+      rewrite 2 dom_fmap, 2 dom_kmap_L' in Hdisj'.
+      intros ->.
+      now apply Hdisj' in Hb.
+  }
+  rewrite relabel_sized_graph_Pmap_map_to_Pmap_injmap. 2:{
+    rewrite 3 (vertices_reindex_sized_graph _).
+    rewrite vertices_swapped_stack_sized_graphs_aux by done.
+    now rewrite dom_union_L, 2 dom_fun_to_map_L.
+  }
+  constructor.
+  - apply Pmap_injmap_inj.
+    apply map_inj_disj_union.
+    + now rewrite map_disjoint_dom, 2 dom_fun_to_map_L,
+      2 (vertices_reindex_sized_graph _).
+    + now apply fun_to_map_inj.
+    + now apply fun_to_map_inj.
+    + intros i j a b Ha%(elem_of_map_img_2 (SA:=Pset))
+        Hb%(elem_of_map_img_2 (SA:=Pset)).
+      rewrite map_img_fun_to_map_L in Ha, Hb.
+      rewrite (vertices_reindex_sized_graph _) in Ha.
+      rewrite (vertices_reindex_sized_graph _) in Hb.
+      rewrite 2 vertices_relabel_sized_graph, 2 (vertices_reindex_sized_graph _) in Hvdisj'.
+      intros ->.
+      now apply Hvdisj' in Hb.
+  - apply _.
+Qed.
+
+
+Lemma swapped_stack_sized_graphs_aux_to_swapped_stack_sized_graphs_disjoint {n m n' m'}
+  (scohg1 : SizedCospanHyperGraph N T n m) (scohg2 : SizedCospanHyperGraph N T n' m') :
+  hyperedges scohg1 ##ₘ hyperedges scohg2 ->
+  vertices scohg1 ## vertices scohg2 ->
+  sized_isomorphic (swapped_stack_sized_graphs_aux scohg1 scohg2) (swapped_stack_sized_graphs scohg1 scohg2).
+Proof.
+  intros Hdisj Hvdisj.
+  unfold swapped_stack_sized_graphs.
+  apply swapped_stack_sized_graphs_aux_sized_isomorphic.
+  - constructor; apply _.
+  - constructor; apply _.
+  - done.
+  - cbn.
+    apply map_disjoint_fmap.
+    now apply (kmap_inj2_disjoint _).
+  - done.
+  - rewrite 2 vertices_relabel_sized_graph, 2 (vertices_reindex_sized_graph _).
+    set_solver +.
+Qed.
+
+Lemma compose_sized_graphs_aux_to_compose_sized_graphs_disjoint {n m o}
+  (scohg1 : SizedCospanHyperGraph N T n m) (scohg2 : SizedCospanHyperGraph N T m o) :
+  hyperedges scohg1 ##ₘ hyperedges scohg2 ->
+  vertices scohg1 ## vertices scohg2 ->
+  compose_sized_graphs_aux scohg1 scohg2 ≡ᵢ compose_sized_graphs scohg1 scohg2.
+Proof.
+  intros Hdisj Hvdisj.
+  rewrite <- compose_sized_graphs_alt_correct, <- compose_sized_graphs_alt_aux_correct by done.
+  apply sized_add_top_loops_struct_sized_isomorphic.
+  apply (subrel' sized_isomorphic).
+  now apply swapped_stack_sized_graphs_aux_to_swapped_stack_sized_graphs_disjoint.
+Qed.
+
+Lemma sized_isomorphic_reindex_sized_graph {n m} (f : positive -> positive)
+  `{Hf : !Inj eq eq f} (scohg : SizedCospanHyperGraph N T n m) :
+  sized_isomorphic scohg (reindex_sized_graph f scohg).
+Proof.
+  apply sized_isomorphic_exists.
+  exists id, f.
+  rewrite relabel_sized_graph_id.
+  split_and!; [apply _..|done].
+Qed.
+
+Lemma sized_isomorphic_relabel_sized_graph {n m} (f : positive -> positive)
+  `{Hf : !Inj eq eq f} (scohg : SizedCospanHyperGraph N T n m) :
+  sized_isomorphic scohg (relabel_sized_graph f scohg).
+Proof.
+  apply sized_isomorphic_exists.
+  exists f, id.
+  rewrite reindex_sized_graph_id.
+  split_and!; [apply _..|done].
+Qed.
+
+
+Lemma subst_by_vec_notin {n} (v : vec _ n) p :
+  p ∉ v.*1 ->
+  subst_by_vec v p = p.
+Proof.
+  revert p; induction v as [|(i, o) n v IHv]; intros p; [done|].
+  cbn.
+  intros Hp.
+  rewrite fn_lookup_singleton_ne by now intros ->; apply Hp; left.
+  apply IHv.
+  eauto using elem_of_list.
+Qed.
+
+(* FIXME: Move *)
+Lemma Pmap_map_insert k v m p :
+  Pmap_map (<[k := v]> m) p = <[k := v]> (Pmap_map m) p.
+Proof.
+  unfold Pmap_map.
+  rewrite lookup_insert_case, fn_lookup_insert_case.
+  case_decide; done.
+Qed.
+
+Lemma subst_by_vec_disj {n} (v : vec _ n) p :
+  v.*1 ## v.*2 ->
+  subst_by_vec v p =
+  Pmap_map (list_to_map v :> Pmap positive) p.
+Proof.
+  revert p; induction v as [|(i, o) n v IHv]; intros p.
+  - cbn.
+    unfold Pmap_map.
+    now rewrite lookup_empty.
+  - cbn.
+    intros Hdisj.
+    rewrite fn_lookup_singleton_case.
+    rewrite Pmap_map_insert, fn_lookup_insert_case.
+    case_decide as Hip.
+    + subst p.
+      now rewrite subst_by_vec_notin by set_solver +Hdisj.
+    + apply IHv.
+      intros k Hk1 Hk2.
+      apply (Hdisj k); now constructor.
+Qed.
+
+
+Lemma subst_by_vec_case {n} (v : vec _ n) p :
+  (p ∈ v.*1 /\ subst_by_vec v p ∈ v.*2) \/
+  (p ∉ v.*1 /\ subst_by_vec v p = p).
+Proof.
+  revert p.
+  induction n as [|n IHn]; [induction v using vec_0_inv; right; split; easy|].
+  intros p.
+  induction v as [(i, o) v] using vec_S_inv.
+  cbn.
+  rewrite fn_lookup_singleton_case.
+  case_decide as Hip.
+  - left.
+    subst p.
+    split; [constructor|].
+    destruct (IHn v o) as [[? ?]|[? ->]];
+    eauto using elem_of_list.
+  - destruct (IHn v p) as [[? ?]|[? ->]];
+    [eauto using elem_of_list|].
+    right.
+    split; [|done].
+    now rewrite not_elem_of_cons.
+Qed.
+
+(* FIXME: Move *)
+Lemma fn_lookup_singleton_ne_strong `{EqDecision A} (a b c : A) :
+  (a <> b -> a <> c) ->
+  {[a := b]} c = c.
+Proof.
+  rewrite fn_lookup_singleton_case.
+  case_decide; [|done].
+  destruct_decide (decide (a = b)); [now subst|tauto].
+Qed.
+Lemma fn_lookup_singleton_idemp `{EqDecision A} (a b c : A) :
+  {[a := b]} ({[a := b]} c) =@{A} {[a := b]} c.
+Proof.
+  rewrite 2 fn_lookup_singleton_case.
+  destruct_decide (decide (a = c)); case_decide; congruence.
+Qed.
+
+
+Lemma snds_propogate_subst_subseteq {n} (v : vec _ n) :
+  (propogate_subst v).*2 ⊆ v.*2.
+Proof.
+  induction n as [|n IHn]; [now induction v using vec_0_inv|].
+  induction v as [(i, o) v] using vec_S_inv.
+  cbn.
+  rewrite list_subseteq_cons_iff.
+  split; [constructor|].
+  rewrite IHn.
+  rewrite vec_to_list_map.
+  rewrite snds_prod_map.
+  intros _k (k & -> & Hk)%elem_of_list_fmap.
+  rewrite fn_lookup_singleton_case.
+  case_decide; [constructor|].
+  now constructor.
+Qed.
+
+
+Lemma subst_by_vec_propogate_subst_idemp {n} (v : vec _ n) p :
+  subst_by_vec (propogate_subst v) (subst_by_vec (propogate_subst v) p) =
+  subst_by_vec (propogate_subst v) p.
+Proof.
+  revert p;
+  induction n as [|n IHn]; [now induction v using vec_0_inv|].
+  intros p.
+  induction v as [(i, o) v] using vec_S_inv.
+  cbn.
+  rewrite (fn_lookup_singleton_case _ _ p).
+  case_decide as Hip.
+  - subst p.
+    rewrite fn_lookup_singleton_ne_strong; [apply IHn|].
+    intros Hio.
+    symmetry.
+    destruct (subst_by_vec_case
+      (propogate_subst (vmap (prod_map {[i := o]} {[i := o]}) v)) o)
+      as [[_ Hin]|[_ ->]]; [|done].
+    intros Heq.
+    rewrite Heq in Hin.
+    apply snds_propogate_subst_subseteq in Hin.
+    rewrite vec_to_list_map, snds_prod_map in Hin.
+    apply elem_of_list_fmap in Hin as (k & Hk & _).
+    rewrite fn_lookup_singleton_case in Hk.
+    case_decide; done.
+  - rewrite fn_lookup_singleton_ne_strong; [apply IHn|].
+    intros Hio.
+    symmetry.
+    destruct (subst_by_vec_case
+      (propogate_subst (vmap (prod_map {[i := o]} {[i := o]}) v)) p)
+      as [[_ Hin]|[_ ->]]; [|done].
+    intros Heq.
+    rewrite Heq in Hin.
+    apply snds_propogate_subst_subseteq in Hin.
+    rewrite vec_to_list_map, snds_prod_map in Hin.
+    apply elem_of_list_fmap in Hin as (k & Hk & _).
+    rewrite fn_lookup_singleton_case in Hk.
+    case_decide; done.
+Qed.
+
+(* Lemma subst_by_vec_propogate_subst_do_subst {n} (v : vec (positive * positive) n)
+  i o p :
+  (i, o) ∈ vec_to_list v ->
+  subst_by_vec (propogate_subst v) p =
+  subst_by_vec (propogate_subst v) ({[i := o]} p).
+Proof.
+  revert i o p;
+  induction n as [|n IHn]; [now induction v using vec_0_inv|].
+  induction v as [(i', o') v] using vec_S_inv.
+  intros i o p.
+  cbn [vec_to_list].
+  rewrite elem_of_cons.
+  intros [[= <- <-]| Hio];
+  [cbn; now rewrite fn_lookup_singleton_idemp|].
+   *)
+
+Lemma subst_by_vec_filter_not_id {n} (v : vec _ n) p :
+  subst_by_vec v p =
+  subst_by_vec (list_to_vec (filter (λ io, io.1 <> io.2) (vec_to_list v))) p.
+Proof.
+  revert p; induction v as [|(i, o) n v IHv]; [done|].
+  intros p.
+  cbn.
+  case_decide; [cbn; apply IHv|].
+  subst.
+  rewrite fn_lookup_singleton_id.
+  apply IHv.
+Qed.
+
+Lemma subst_by_vec_helper_bcons_true_id {n}
+  (v : vec _ n) p :
+  Forall (fun io =>
+    io.1 = io.2 \/ (io.1 = bcons false (pos_tail io.1)
+      /\ io.2 = bcons true (pos_tail io.1))) v ->
+  subst_by_vec v (bcons true p) = bcons true p.
+Proof.
+  intros Hall.
+  rewrite subst_by_vec_filter_not_id.
+  apply subst_by_vec_notin.
+  rewrite not_elem_of_list_fmap.
+  intros io Hio.
+  rewrite vec_to_list_to_vec in Hio.
+  apply elem_of_list_filter in Hio as [Hio Hiov].
+  rewrite Forall_forall in Hall.
+  apply Hall in Hiov as [|[Hio1 Hio2]]; [done|].
+  rewrite Hio1.
+  lia.
+Qed.
+
+(* Lemma propogate_subst_disj_alt {n} (v : vec _ n) :
+  Forall (λ io, io.1 = io.2 \/ io.1 ∉ v.*2) v ->
+  propogate_subst v =
+  fun_to_vec (λ i,
+  match list_find (λ io, io.1 = (v !!! i).1) (take i v) with
+  | Some (_, io) => io
+  | None => v !!! i
+  end).
+Proof.
+  induction n as [|n IHn]; [now induction v using vec_0_inv|].
+  induction v as [(i, o) v] using vec_S_inv.
+  cbn [vec_to_list].
+  rewrite Forall_cons.
+  intros [Hio Hv].
+  cbn.
+  f_equal.
+  rewrite IHn.
+  - apply vec_eq; intros p.
+    rewrite 2 lookup_fun_to_vec.
+    rewrite vec_to_list_map.
+    rewrite <- fmap_take, list_find_fmap.
+    cbn.
+  - rewrite vec_to_list_map.
+    rewrite Forall_fmap.
+    rewrite snds_prod_map.
+    rewrite Forall_forall in Hv |- *.
+    intros io' Hio'v.
+    apply Hv in Hio'v as Hio'.
+    cbn in *.
+    simpl.
+    destruct Hio as [-> | Hio].
+    + rewrite 2 fn_lookup_singleton_id.
+      rewrite list_fmap_id' by now intros; rewrite fn_lookup_singleton_id.
+      destruct Hio' as [?|Hio']; [now left|].
+      right.
+      eauto using elem_of_list.
+    + destruct Hio' as [Hio'|Hio']; [now left; f_equal|].
+
+      rewrite fn_lookup_singleton_case.
+
+      case_decide as Hii'.
+      *
+      split; [done|].
+
+    simpl in *.
+    simpl. *)
+
+Lemma vzip_like_vmap {n} i o (v : vec _ n) :
+  Forall (λ io, io.1 = io.2
+     ∨ io.1 = bcons false (pos_tail io.1)
+       ∧ io.2 = bcons true (pos_tail io.1)) ((i, o) :: v) ->
+  Forall (λ io, io.1 = io.2
+     ∨ io.1 = bcons false (pos_tail io.1)
+       ∧ io.2 = bcons true (pos_tail io.1))
+  (vmap (prod_map {[i := o]} {[i := o]}) v).
+Proof.
+  rewrite Forall_cons.
+  intros [Hio Hv].
+  cbn in *.
+  rewrite vec_to_list_map, Forall_fmap.
+  apply (Forall_impl _ _ _ Hv).
+  intros [i' o'].
+  cbn.
+  intros [->|Hio']; [now left; f_equal|].
+  destruct i'; try easy.
+  cbn in *.
+  destruct Hio' as [_ ->].
+  destruct Hio as [->|Hio]; [right; now rewrite 2 fn_lookup_singleton_id|].
+  destruct i; try easy.
+  cbn in Hio.
+  destruct Hio as [_ ->].
+  rewrite fn_lookup_singleton_case.
+  rewrite fn_lookup_singleton_ne by lia.
+  case_decide as Hi; [|by auto].
+  revert Hi.
+  intros [= <-].
+  now left.
+Qed.
+
+
+Lemma propogate_subst_vmap_bcons_false_true_vzip_like {n}
+  (v : vec _ n) :
+  Forall (fun io =>
+    io.1 = io.2 \/ (io.1 = bcons false (pos_tail io.1)
+      /\ io.2 = bcons true (pos_tail io.1))) v ->
+  Forall (fun io =>
+    io.1 = io.2 \/ (io.1 = bcons false (pos_tail io.1)
+      /\ io.2 = bcons true (pos_tail io.1)))
+    (propogate_subst v).
+Proof.
+  induction n as [|n IHn]; [now induction v using vec_0_inv|].
+  induction v as [(i, o) v] using vec_S_inv.
+  cbn.
+  rewrite 2 Forall_cons.
+  cbn.
+  intros [Hio Hv].
+  split; [exact Hio|].
+  apply IHn.
+  clear IHn.
+  now apply vzip_like_vmap, Forall_cons.
+Qed.
+
+
+
+
+
+(*
+Lemma propogate_subst_vmap_bcons_false_true_vzip {n}
+  (v : vec positive n) :
+  propogate_subst
+    (vmap (prod_map (bcons false) (bcons true))
+      (vzip v v)) =
+  fun_to_vec (λ i,
+  if decide (v !!! i ∈ take i v) then
+    (bcons true $ Pos.of_succ_nat i, bcons true $ Pos.of_succ_nat i)
+  else
+    (bcons false $ Pos.of_succ_nat i, bcons true $ Pos.of_succ_nat i)).
+Proof. *)
+
+
+
+Lemma vzip_like_vmap_strong {n} i o (v : vec _ n) :
+  Forall (λ io, (io.1 = io.2
+     ∨ io.1 = bcons false (pos_tail io.1))
+       ∧ io.2 = bcons true (pos_tail io.1)) ((i, o) :: v) ->
+  Forall (λ io, (io.1 = io.2
+     ∨ io.1 = bcons false (pos_tail io.1))
+       ∧ io.2 = bcons true (pos_tail io.1))
+  (vmap (prod_map {[i := o]} {[i := o]}) v).
+Proof.
+  rewrite Forall_cons.
+  intros [Hio Hv].
+  cbn in *.
+  rewrite vec_to_list_map, Forall_fmap.
+  apply (Forall_impl _ _ _ Hv).
+  intros [i' o'].
+  cbn.
+  intros [[->|Hio'] Ho'].
+  - split; [now left; f_equal|].
+    destruct Hio as [[-> | ->] Ho]; [now rewrite fn_lookup_singleton_id|].
+    cbn.
+    rewrite Ho'.
+    rewrite fn_lookup_singleton_ne by lia.
+    done.
+  - destruct i'; try easy.
+    cbn in *.
+    subst o'.
+    destruct Hio as [[-> | Hi] Hio]; [now rewrite !fn_lookup_singleton_id; auto|].
+    destruct i; try easy.
+    cbn in Hio.
+    subst o.
+    rewrite fn_lookup_singleton_case.
+    rewrite fn_lookup_singleton_ne by lia.
+    case_decide as Hii'; [|by auto].
+    revert Hii'.
+    intros [= <-].
+    auto.
+Qed.
+
+
+Lemma propogate_subst_vmap_bcons_false_true_vzip_like_strong {n}
+  (v : vec _ n) :
+  Forall (λ io, (io.1 = io.2
+     ∨ io.1 = bcons false (pos_tail io.1))
+       ∧ io.2 = bcons true (pos_tail io.1)) v ->
+  Forall (λ io, (io.1 = io.2
+     ∨ io.1 = bcons false (pos_tail io.1))
+       ∧ io.2 = bcons true (pos_tail io.1))
+    (propogate_subst v).
+Proof.
+  induction n as [|n IHn]; [now induction v using vec_0_inv|].
+  induction v as [(i, o) v] using vec_S_inv.
+  cbn.
+  rewrite 2 Forall_cons.
+  cbn.
+  intros [Hio Hv].
+  split; [exact Hio|].
+  apply IHn.
+  clear IHn.
+  now apply vzip_like_vmap_strong, Forall_cons.
+Qed.
+
+
+Lemma propogate_subst_vmap_bcons_false_true_vzip {n}
+  (v : vec positive n) :
+  Forall (fun io =>
+    io.1 = io.2 \/ (io.1 = bcons false (pos_tail io.1)
+      /\ io.2 = bcons true (pos_tail io.1)))
+    (propogate_subst
+    (vmap (prod_map (bcons false) (bcons true))
+      (vzip v v))).
+Proof.
+  apply propogate_subst_vmap_bcons_false_true_vzip_like.
+  rewrite vec_to_list_map, vec_to_list_zip_with.
+  rewrite Forall_fmap, Forall_lookup.
+  intros k (i, o) Hio%lookup_zip_Some.
+  assert (i = o) as -> by now destruct Hio; congruence.
+  simpl.
+  now right.
+Qed.
+
+
+Lemma subst_by_vec_helper_bcons_false {n}
+  (v : vec _ n) p :
+  Forall (λ io, (io.1 = io.2
+     ∨ io.1 = bcons false (pos_tail io.1))
+       ∧ io.2 = bcons true (pos_tail io.1)) v ->
+  subst_by_vec v (bcons false p) =
+  if decide (bcons false p ∈ (vec_to_list v).*1)
+    then bcons true p else bcons false p.
+Proof.
+  intros Hall.
+  revert p; induction n as [|n IHn]; [now induction v using vec_0_inv|].
+  intros p.
+  induction v as [(i, o) v] using vec_S_inv.
+  cbn in *.
+  apply Forall_cons in Hall as Hall'.
+  destruct Hall' as [Hio Hv].
+  cbn in Hio.
+  destruct Hio as [[<-|Hi] Ho].
+  - rewrite fn_lookup_singleton_id.
+    rewrite IHn by done.
+    apply decide_ext.
+    rewrite elem_of_cons.
+    enough(p~0 <> i) by tauto.
+    now destruct i.
+  - subst o.
+    destruct i; try now contradict Hi.
+    cbn.
+    rewrite fn_lookup_singleton_case.
+    rewrite (decide_ext _ _ _ _ (inj_iff xO i p)).
+    case_decide as Hip.
+    + subst p.
+      rewrite decide_True by constructor.
+      apply subst_by_vec_helper_bcons_true_id.
+      apply (Forall_impl _ _ _ Hv).
+      intros [i' o'].
+      cbn.
+      destruct o'; try easy.
+      cbn.
+      destruct i'; cbn; firstorder congruence.
+    + rewrite IHn by done.
+      apply decide_ext.
+      rewrite elem_of_cons.
+      enough(p~0 <> i~0) by tauto.
+      congruence.
+Qed.
+
+(* FIXME: Move *)
+Lemma list_subseteq_antisymm {A} (l l' : list A) :
+  l ⊆ l' -> l' ⊆ l -> l ≡ l'.
+Proof.
+  firstorder.
+Qed.
+
+Lemma fsts_propogate_subst_subseteq {n} (v : vec _ n) :
+  (propogate_subst v).*1 ⊆ v.*1 ++ v.*2.
+Proof.
+  induction n as [|n IHn]; [now induction v using vec_0_inv|].
+  induction v as [(i, o) v] using vec_S_inv.
+  cbn.
+  rewrite list_subseteq_cons_iff.
+  split; [now constructor|].
+  rewrite IHn.
+  rewrite vec_to_list_map, fsts_prod_map, snds_prod_map.
+  clear IHn.
+  intros k.
+  rewrite elem_of_app.
+  rewrite 2 elem_of_list_fmap.
+  setoid_rewrite fn_lookup_singleton_case.
+  firstorder case_decide; set_solver.
+Qed.
+
+Lemma fsts_propogate_subst_supseteq {n} (v : vec _ n) :
+  v.*1 ⊆ (propogate_subst v).*1.
+Proof.
+  induction n as [|n IHn]; [now induction v using vec_0_inv|].
+  induction v as [(i, o) v] using vec_S_inv.
+  cbn.
+  rewrite list_subseteq_cons_iff.
+  split; [now constructor|].
+  etransitivity. 2:{
+    apply list_subseteq_skip.
+    apply IHn.
+  }
+  rewrite vec_to_list_map, fsts_prod_map.
+  intros k.
+  rewrite elem_of_cons.
+  rewrite (elem_of_list_fmap {[_:=_]}).
+  setoid_rewrite fn_lookup_singleton_case.
+  intros Hk.
+  destruct_decide (decide (k = i)); [now left|].
+  right.
+  exists k.
+  rewrite decide_False by done.
+  done.
+Qed.
+
+Lemma subst_by_vec_propogate_subst_vmap_bcons_false_true_vzip {n}
+  (v : vec positive n) p :
+  subst_by_vec (propogate_subst
+    (vmap (prod_map (bcons false) (bcons true)) (vzip v v)))
+    (bcons false p) =
+  if decide (p ∈ vec_to_list v) then bcons true p else bcons false p.
+Proof.
+  rewrite subst_by_vec_helper_bcons_false.
+  - apply decide_ext.
+    split. 2:{
+      intros Hp.
+      apply fsts_propogate_subst_supseteq.
+      rewrite vec_to_list_map, fsts_prod_map.
+      apply elem_of_list_fmap_1.
+      rewrite vec_to_list_zip_with.
+      now rewrite fst_zip by done.
+    }
+    intros Hp%fsts_propogate_subst_subseteq.
+    rewrite vec_to_list_map, fsts_prod_map, snds_prod_map,
+      vec_to_list_zip_with, fst_zip, snd_zip in Hp by done.
+    set_solver.
+  - apply propogate_subst_vmap_bcons_false_true_vzip_like_strong.
+    rewrite vec_to_list_map, Forall_fmap.
+    rewrite vec_to_list_zip_with.
+    rewrite Forall_zip_with by done.
+    apply Forall_Forall2_diag.
+    rewrite Forall_forall.
+    auto.
+Qed.
+
+Lemma compose_sized_graphs_unsafe_to_compose_sized_graphs {n m o}
+  (tgl : SizedCospanHyperGraph N T n m) (tgr : SizedCospanHyperGraph N T m o) :
+  tgl.(outputs) = tgr.(inputs) ->
+  vertices tgl ∖ list_to_set (outputs tgl) ##
+  vertices tgr ∖ list_to_set (inputs tgr) ->
+  hyperedges tgl ##ₘ hyperedges tgr ->
+  compose_sized_graphs_unsafe tgl tgr ≡ᵢ compose_sized_graphs tgl tgr.
+Proof.
+  intros Hoi Hvdisj Hdisj.
+  rewrite <- compose_sized_graphs_aux_to_compose_sized_graphs_unsafe by done.
+  rewrite <- compose_sized_graphs_alt_aux_correct by done.
+  rewrite <- compose_sized_graphs_alt_correct.
+  apply sized_add_top_loops_struct_sized_isomorphic_strong.
+  cbn.
+  rewrite 4 vsplitl_app.
+  transitivity (relabel_sized_graph
+     (subst_by_vec
+        (propogate_subst
+           (vzip (vmap (bcons false) (outputs tgl))
+              (vmap (bcons true) (inputs tgr)))))
+     (swapped_stack_sized_graphs_aux (relabel_sized_graph (bcons false) tgl)
+      (relabel_sized_graph (bcons true) tgr))). 2:{
+    set (f := (fun i => if decide (i ∈ dom (hyperedges tgl)) then bcons false i else bcons true i)).
+    assert (Hf : Inj eq eq f). 1:{
+      intros i j.
+      unfold f.
+      do 2 case_decide; now intros ?%(inj2 bcons).
+    }
+    rewrite (sized_isomorphic_reindex_sized_graph f).
+    apply eq_reflexivity.
+    rewrite reindex_relabel_sized_graph.
+    rewrite reindex_swapped_stack_sized_graphs_aux by apply _.
+    f_equal.
+    unfold swapped_stack_sized_graphs.
+    rewrite 2 reindex_relabel_sized_graph.
+    f_equal; f_equal.
+    - apply reindex_sized_graph_ext_strong.
+      intros i _ Hi%elem_of_dom_2.
+      unfold f.
+      now rewrite decide_True by done.
+    - apply reindex_sized_graph_ext_strong.
+      intros i _ Hi%elem_of_dom_2.
+      unfold f.
+      rewrite map_disjoint_dom in Hdisj.
+      now rewrite decide_False by now intros ?%Hdisj.
+  }
+  set (f := (fun i =>
+    if decide (i ∈ vertices tgl ∖ list_to_set (outputs tgl)) then
+    bcons false i else bcons true i)).
+  assert (Hf : Inj eq eq f). 1:{
+    intros i j.
+    unfold f.
+    do 2 case_decide; now intros ?%(inj2 bcons).
+  }
+  rewrite (sized_isomorphic_relabel_sized_graph f).
+  rewrite relabel_sized_graph_compose, 2 relabel_swapped_stack_sized_graphs_aux,
+    2 relabel_sized_graph_compose.
+  apply eq_reflexivity.
+  f_equal.
+  - apply relabel_sized_graph_ext_strong.
+    intros i Hi.
+    cbn.
+    rewrite Hoi.
+    rewrite vzip_map.
+    rewrite subst_by_vec_id.
+    rewrite subst_by_vec_propogate_subst_vmap_bcons_false_true_vzip.
+    case_decide as Hii.
+    + cbn.
+      unfold f.
+      now rewrite Hoi, decide_False by now rewrite elem_of_difference, elem_of_list_to_set.
+    + unfold f.
+      now rewrite Hoi, decide_True by now rewrite elem_of_difference, elem_of_list_to_set.
+  - apply relabel_sized_graph_ext_strong.
+    intros i Hi.
+    cbn.
+    rewrite Hoi.
+    rewrite vzip_map.
+    rewrite subst_by_vec_id.
+    rewrite subst_by_vec_helper_bcons_true_id by
+      apply propogate_subst_vmap_bcons_false_true_vzip.
+    unfold f.
+    case_decide as Hii; [|done].
+    apply Hvdisj in Hii as Hii'.
+    rewrite elem_of_difference in Hii, Hii'.
+    rewrite Hoi in Hii.
+    tauto.
+Qed.
+
+
+Lemma compose_sized_graphs_unsafe'_to_compose_sized_graphs {n m o}
+  (tgl : SizedCospanHyperGraph N T n m) (tgr : SizedCospanHyperGraph N T m o) :
+  tgl.(outputs) = tgr.(inputs) ->
+  vertices tgl ∖ list_to_set (outputs tgl) ##
+  vertices tgr ∖ list_to_set (inputs tgr) ->
+  hyperedges tgl ##ₘ hyperedges tgr ->
+  compose_sized_graphs_unsafe' tgl tgr ≡ᵢ compose_sized_graphs tgl tgr.
+Proof.
+  intros.
+  etransitivity.
+  - apply (subrel' scohg_vert_eq).
+    apply compose_sized_graphs_unsafe'_correct.
+  - now apply compose_sized_graphs_unsafe_to_compose_sized_graphs.
+Qed.
+
+
+
+
+Lemma stack_sized_graphs_id_0_l {n m} (scohg : SizedCospanHyperGraph N T n m) :
+  stack_sized_graphs (id_sized_graph 0) scohg ≡ᵢ scohg.
+Proof.
+  symmetry.
+  rewrite (sized_iso_relabel_reindex _ xI xI) at 1.
+  apply eq_reflexivity.
+  unfold stack_sized_graphs, stack_sized_graphs_aux.
+  cbn.
+  change (relabel_hg (bcons false) _) with (∅ :> HyperGraph T).
+  apply scohg_ext; [|done..].
+  cbn.
+  apply hg_ext; [|set_solver].
+  symmetry.
+  apply map_empty_union.
+Qed.
+
+Lemma empty_sized_graph_0_0_eq {n m} (scohg scohg' : SizedCospanHyperGraph N T n m) :
+  scohg.(hedges) = ∅ ->
+  scohg'.(hedges) = ∅ ->
+  n = 0 -> m = 0 ->
+  scohg = scohg'.
+Proof.
+  destruct scohg, scohg'; cbn.
+  intros; subst.
+  inv_all_vec_fin; f_equal; done.
+Qed.
+
+Lemma delta_spider_sized_graph_alt n m k :
+  sized_isomorphic (T:=T) (delta_spider_sized_graph n m)
+    (mk_scohg (mk_hg ∅ {[k]}) (fun_to_vec (λ _, k)) (fun_to_vec (λ _, k))).
+Proof.
+  rewrite (sized_iso_relabel_reindex (delta_spider_sized_graph n m) (λ p, pos_add_N p (Pos.pred_N k)) id
+    (Hfe:=(ltac:(intros ? ?; lia)))).
+  apply eq_reflexivity.
+  apply scohg_ext.
+  - apply hg_ext; [done|].
+    cbn -[set_map].
+    rewrite set_map_singleton_L.
+    f_equal; lia.
+  - apply vec_eq; intros i.
+    cbn.
+    rewrite vlookup_map, 2 lookup_fun_to_vec.
+    lia.
+  - apply vec_eq; intros i.
+    cbn.
+    rewrite vlookup_map, 2 lookup_fun_to_vec.
+    lia.
+Qed.
+
+Lemma n_stack_delta_spider_sized_graph_alt k n m :
+  forall offset,
+  n_stack_sized_graphs k (delta_spider_sized_graph (T:=T) n m) ≡ᵢ
+  mk_scohg (mk_hg ∅ (list_to_set (Pos.of_succ_nat <$> seq offset k)))
+    (fun_to_vec (λ i, Pos.of_succ_nat (offset + i / n)))
+    (fun_to_vec (λ i, Pos.of_succ_nat (offset + i / m))).
+Proof.
+  induction k; [done|].
+  cbn.
+  intros offset.
+  rewrite (delta_spider_sized_graph_alt n m (Pos.of_succ_nat offset)) at 1.
+  rewrite (IHk (S offset)).
+  rewrite <- stack_sized_graphs_aux_to_stack_sized_graphs_disjoint; [|done|].
+  2:{
+    rewrite vertices_almost_empty_sized_graph.
+    rewrite vec_to_list_app, 2 (vec_to_list_fun_to_vec (λ _, Pos.of_succ_nat offset)).
+    rewrite list_to_set_app.
+    rewrite 2 (fmap_const _ (Pos.of_succ_nat offset)).
+    rewrite vertices_almost_empty_sized_graph.
+    rewrite vec_to_list_app, 2 (vec_to_list_fun_to_vec (λ i, Pos.of_succ_nat (_ + (i / _)))).
+    set_unfold.
+    intros ?.
+    rewrite 2 elem_of_replicate.
+    setoid_rewrite elem_of_seq.
+    set_unfold; naive_solver lia.
+  }
+  apply eq_reflexivity.
+  apply scohg_ext.
+  - done.
+  - cbn.
+    rewrite fun_to_vec_plus.
+    f_equal.
+    + apply fun_to_vec_ext_mor.
+      intros i.
+      cbn.
+      rewrite fin_to_nat_L.
+      rewrite Nat.div_small by apply fin_to_nat_lt.
+      lia.
+    + apply fun_to_vec_ext_mor.
+      intros i.
+      cbn.
+      rewrite fin_to_nat_R.
+      rewrite <- (Nat.mul_1_l n) at 3.
+      rewrite Nat.div_add_l by (pose proof (fin_to_nat_lt i); lia).
+      lia.
+  - cbn.
+    rewrite fun_to_vec_plus.
+    f_equal.
+    + apply fun_to_vec_ext_mor.
+      intros i.
+      cbn.
+      rewrite fin_to_nat_L.
+      rewrite Nat.div_small by apply fin_to_nat_lt.
+      lia.
+    + apply fun_to_vec_ext_mor.
+      intros i.
+      cbn.
+      rewrite fin_to_nat_R.
+      rewrite <- (Nat.mul_1_l m) at 3.
+      rewrite Nat.div_add_l by (pose proof (fin_to_nat_lt i); lia).
+      lia.
+Qed.
+
+Lemma permute_sized_graph_relabel_sized_graph {n m n' m'}
+  (fl : fin n -> fin n') {Hfl : Inj eq eq fl}
+  (fr : fin m -> fin m') {Hfr : Inj eq eq fr}
+  (Hn : n = n') (Hm : m = m') f (scohg : SizedCospanHyperGraph N T n m) :
+  permute_sized_graph fl fr (relabel_sized_graph f scohg) = relabel_sized_graph f (permute_sized_graph fl fr scohg).
+Proof.
+  subst.
+  rewrite 2 (permute_sized_graph_alt fl fr).
+  apply scohg_ext; [done|..].
+  - cbn.
+    apply vec_eq.
+    intros i.
+    rewrite vlookup_map, 2 lookup_permute_vec, vlookup_map.
+    done.
+  - cbn.
+    apply vec_eq.
+    intros i.
+    rewrite vlookup_map, 2 lookup_permute_vec, vlookup_map.
+    done.
+Qed.
+
+Lemma permute_sized_graph_reindex_sized_graph {n m n' m'}
+  (fl : fin n -> fin n')
+  (fr : fin m -> fin m')  f (scohg : SizedCospanHyperGraph N T n m) :
+  permute_sized_graph fl fr (reindex_sized_graph f scohg) = reindex_sized_graph f (permute_sized_graph fl fr scohg).
+Proof.
+  done.
+Qed.
+
+Lemma permute_sized_graph_sized_isomorphic {n m n' m'}
+  (fl : fin n -> fin n') {Hfl : Inj eq eq fl}
+  (fr : fin m -> fin m') {Hfr : Inj eq eq fr}
+  (Hn : n = n') (Hm : m = m') : Proper (sized_isomorphic ==> sized_isomorphic) (permute_sized_graph (T:=T) fl fr).
+Proof.
+  subst.
+  intros scohg scohg' Heq.
+  induction Heq as [scohg fv fe Hfv Hfe].
+  rewrite (permute_sized_graph_relabel_sized_graph fl fr), permute_sized_graph_reindex_sized_graph by done.
+  now constructor.
+Qed.
+
+#[export] Instance permute_sized_graph_scohg_vert_eq {n m n' m'}
+  (fl : fin n -> fin n') {Hfl : Inj eq eq fl}
+  (fr : fin m -> fin m') {Hfr : Inj eq eq fr}
+  (Hn : n = n') (Hm : m = m') :
+  Proper (scohg_vert_eq ==> scohg_vert_eq) (permute_sized_graph (T:=T) fl fr).
+Proof.
+  intros scohg scohg' Heq.
+  rewrite scohg_vert_eq_alt_vertices in Heq.
+  rewrite scohg_vert_eq_alt_vertices.
+  subst.
+  rewrite 2 (vertices_permute_sized_graph fl fr).
+  cbn.
+  destruct Heq as (<- & <- & <- & <-).
+  done.
+Qed.
+
+#[export] Instance permute_sized_graph_struct_sized_isomorphic {n m n' m'}
+  (fl : fin n -> fin n') {Hfl : Inj eq eq fl}
+  (fr : fin m -> fin m') {Hfr : Inj eq eq fr}
+  (Hn : n = n') (Hm : m = m') :
+  Proper (struct_sized_isomorphic ==> struct_sized_isomorphic) (permute_sized_graph (T:=T) fl fr).
+Proof.
+  apply proper_struct_sized_isomorphic_of_vert_eq_unary.
+  - now apply permute_sized_graph_scohg_vert_eq.
+  - now apply permute_sized_graph_sized_isomorphic.
+Qed.
+
+(* FIXME: Move *)
+Lemma fin_perm_cancel_comm {n} (f g : fin n -> fin n)
+  (Hfg : Cancel eq f g) : Cancel eq g f.
+Proof.
+  intros x.
+  assert (Hg : Inj eq eq g) by apply cancel_inj.
+  apply finite.finite_inj_surj in Hg as Hg'; [|done].
+  destruct (Hg' x) as [y Hy].
+  apply (f_equal f) in Hy as Hy'.
+  rewrite Hfg in Hy'.
+  congruence.
+Qed.
+
+Lemma fin_perm_inv_cancel {n} (f g : fin n -> fin n)
+  {Hfg : Cancel eq f g} : Cancel eq (fin_perm_inv f) (fin_perm_inv g).
+Proof.
+  apply fin_perm_cancel_comm in Hfg as Hgf.
+  assert (Hf : Inj eq eq f) by apply cancel_inj.
+  assert (Hg : Inj eq eq g) by apply cancel_inj.
+  intros i.
+  rewrite (fin_perm_inv_spec _).
+  symmetry.
+  rewrite (fin_perm_inv_spec _).
+  apply Hgf.
+Qed.
+
+Lemma permute_sized_graph_alt_cancel {n m n' m'}
+  (fl : fin n -> fin n') (gl : fin n' -> fin n)
+  (fr : fin m -> fin m') (gr : fin m' -> fin m)
+  {Hfgl : Cancel eq fl gl} {Hfgr : Cancel eq fr gr}
+  (Hn : n = n') (Hm : m = m') (scohg : SizedCospanHyperGraph N T n m) :
+  permute_sized_graph fl fr scohg =
+  mk_scohg scohg
+    (permute_vec gl scohg.(inputs))
+    (permute_vec gr scohg.(outputs)).
+Proof.
+  subst.
+  pose proof @cancel_inj.
+  apply fin_perm_cancel_comm in Hfgl as ?.
+  apply fin_perm_cancel_comm in Hfgr as ?.
+  rewrite (permute_sized_graph_alt fl fr).
+  f_equal; apply permute_vec_ext, reflexivity.
+  - intros i.
+    apply (fin_perm_inv_spec fl).
+    apply Hfgl.
+  - intros i.
+    apply (fin_perm_inv_spec fr).
+    apply Hfgr.
+Qed.
+
+
+
+Lemma delta_spider_sized_graph_bundled_alt k n m :
+  delta_spider_sized_graph_bundled (T:=T) k n m ≡ᵢ
+  copy_sized_graph k (delta_spider_sized_graph n m).
+Proof.
+  unfold copy_sized_graph.
+  erewrite (permute_sized_graph_struct_sized_isomorphic fin_prod_comm fin_prod_comm
+    (Nat.mul_comm _ _) (Nat.mul_comm _ _) _) by
+    (apply (n_stack_delta_spider_sized_graph_alt _ _ _ 0)).
+  rewrite (permute_sized_graph_alt_cancel _ _ _ _) by lia.
+  apply eq_reflexivity.
+  apply scohg_ext.
+  - done.
+  - apply vec_eq.
+    intros i.
+    cbn.
+    rewrite lookup_permute_vec, 2 lookup_fun_to_vec.
+    pose proof fin_to_nat_lt i.
+    induction i as [il ir] using fin_mul_ind.
+    rewrite fin_prod_comm_prod.
+    rewrite 2 fin_to_nat_prod.
+    rewrite Nat.div_add_l by lia.
+    rewrite (Nat.add_comm (_ * _) _), Nat.Div0.mod_add.
+    pose proof fin_to_nat_lt il.
+    pose proof fin_to_nat_lt ir.
+    rewrite Nat.div_small, Nat.mod_small by lia.
+    lia.
+  - apply vec_eq.
+    intros i.
+    cbn.
+    rewrite lookup_permute_vec, 2 lookup_fun_to_vec.
+    pose proof fin_to_nat_lt i.
+    induction i as [il ir] using fin_mul_ind.
+    rewrite fin_prod_comm_prod.
+    rewrite 2 fin_to_nat_prod.
+    rewrite Nat.div_add_l by lia.
+    rewrite (Nat.add_comm (_ * _) _), Nat.Div0.mod_add.
+    pose proof fin_to_nat_lt il.
+    pose proof fin_to_nat_lt ir.
+    rewrite Nat.div_small, Nat.mod_small by lia.
+    lia.
+Qed.
+
+End StackCompose.
+
+
+
+
+
+
+Lemma hypergraph_empty_union {T} (hg : HyperGraph T) : ∅ ∪ hg = hg.
+Proof.
+  apply hg_ext.
+  - apply map_empty_union.
+  - unfold union, hypergraph_union.
+    cbn -[union].
+    apply union_empty_l_L.
+Qed.
+
+(* FIXME: Move *)
+Lemma vmap_vzip_with {A B C D} (f : C -> D) (g : A -> B -> C) {n}
+  (v w : vec _ n) :
+  vmap f (vzip_with g v w) = vzip_with (λ a b, f (g a b)) v w.
+Proof.
+  induction n; inv_all_vec_fin; cbn in *; congruence.
+Qed.
+Lemma fst_vzip {A} {n} (v w : vec A n) :
+  vmap fst (vzip_with pair v w) = v.
+Proof.
+  induction n; inv_all_vec_fin; cbn in *; congruence.
+Qed.
+Lemma snd_vzip {A} {n} (v w : vec A n) :
+  vmap snd (vzip_with pair v w) = w.
+Proof.
+  induction n; inv_all_vec_fin; cbn in *; congruence.
+Qed.
+
+Lemma propogate_subst_vmap_bcons_false_true_NoDup_l
+  {n} (v w : vec positive n) : NoDup v ->
+  propogate_subst (vmap (prod_map (bcons false) (bcons true)) (vzip v w)) =
+  vmap (prod_map (bcons false) (bcons true)) (vzip v w).
+Proof.
+  intros Hv.
+  induction n; [inv_all_vec_fin; done|].
+  inv_vec v; intros vh v.
+  inv_vec w; intros wh w.
+  cbn.
+  intros [Hvh Hv]%NoDup_cons.
+  f_equal.
+  rewrite <- IHn at 2 by done.
+  f_equal.
+  apply vmap_id'.
+  intros [k l].
+  rewrite vec_to_list_map, vec_to_list_zip_with.
+  rewrite elem_of_list_fmap.
+  intros ([i j] & [= -> ->] & Hij).
+  apply elem_of_zip_with in Hij as (i' & j' & [= <- <-] & Hi & Hj).
+  cbn.
+  rewrite fn_lookup_singleton_ne by set_solver.
+  rewrite fn_lookup_singleton_ne by lia.
+  done.
+Qed.
+
+
+Lemma compose_sized_graphs_id_sized_graph_l_aux {T n m} (scohg : SizedCospanHyperGraph N T n m) :
+  compose_sized_graphs (id_sized_graph n) scohg ≡ᵥ relabel_sized_graph (bcons true) (reindex_sized_graph (bcons true) scohg).
+Proof.
+  unfold compose_sized_graphs.
+  cbn.
+  rewrite vzip_map.
+  rewrite propogate_subst_vmap_bcons_false_true_NoDup_l by (rewrite vec_to_list_map, vec_to_list_seq;
+    apply (NoDup_fmap _), NoDup_seq).
+  rewrite <- vzip_map.
+  erewrite relabel_sized_graph_ext. 2:{
+    intros i.
+    rewrite subst_by_vec_disj by (rewrite <- 2 vec_to_list_map,
+      fst_vzip, snd_vzip, !vec_to_list_map; set_solver).
+    done.
+  }
+  apply scohg_vert_eq_alt_vertices;
+  split_and!.
+  - cbn.
+    apply vec_eq; intros i.
+    rewrite vlookup_map.
+    unfold Pmap_map.
+    eenough (_ !! _ = Some _) as -> by done.
+    apply elem_of_list_to_map.
+    + rewrite <- vec_to_list_map, fst_vzip, 2 vec_to_list_map, vec_to_list_seq.
+      apply (NoDup_fmap _), (NoDup_fmap _), NoDup_seq.
+    + apply elem_of_vlookup.
+      exists i.
+      rewrite vlookup_zip_with.
+      done.
+  - cbn.
+    apply vmap_id'.
+    rewrite vec_to_list_map.
+    intros _ (i & -> & Hi)%elem_of_list_fmap.
+    unfold Pmap_map.
+    enough (_ !! _ = None) as -> by done.
+    apply not_elem_of_list_to_map.
+    rewrite <- vec_to_list_map, fst_vzip, vec_to_list_map.
+    set_solver.
+  - cbn.
+    rewrite fmap_empty, kmap_empty, map_empty_union.
+    rewrite kmap_fmap'.
+    erewrite map_fmap_ext; [apply map_fmap_id|].
+    intros k [[t i] o].
+    cbn.
+    rewrite lookup_fmap.
+    rewrite fmap_Some.
+    intros ([[t' i'] o'] & _ & [= -> -> ->]).
+    f_equal; [f_equal|]; apply list_fmap_id';
+    intros _ (a & -> & _)%elem_of_list_fmap;
+    unfold Pmap_map;
+    enough (_ !! _ = None) as -> by done;
+    apply not_elem_of_list_to_map;
+    rewrite <- vec_to_list_map, fst_vzip, vec_to_list_map;
+    set_solver.
+  - rewrite vertices_relabel_sized_graph.
+    rewrite 2 vertices_vertices_hg_decomp.
+    cbn.
+    rewrite vertices_hg_add_vertices.
+    unfold disj_union, hypergraph_disjunion.
+    cbn.
+    change (reindex_hg _ (relabel_hg _ ∅)) with (∅ :> HyperGraph T).
+    rewrite hypergraph_empty_union.
+    change (vertices_hg ∅) with (∅ :> Pset).
+    rewrite (union_empty_l_L _).
+    rewrite (vertices_reindex_hg _), vertices_relabel_hg.
+    rewrite (union_comm_L _ (_ ∖ _)).
+    rewrite difference_union_L.
+    rewrite 2 list_to_set_app_L.
+    rewrite vertices_relabel_hg, (vertices_reindex_hg _).
+    etransitivity.
+    1:{
+      apply (f_equal (set_map _)).
+      rewrite (union_comm_L (list_to_set (vmap (bcons false) _))).
+      rewrite union_assoc_L.
+      rewrite (union_comm_L _ (set_map _ _)).
+      rewrite <- (union_assoc_L (set_map _ _)).
+      done.
+    }
+    rewrite set_map_union_L.
+    etransitivity; [apply f_equal2|].
+    1:{
+      erewrite set_map_ext_L; [apply set_map_id_L|].
+      intros x Hx.
+      assert (exists i, x = i~1) as [i ->]. 1:{
+        rewrite 2 vec_to_list_map in Hx.
+        rewrite <- 2 (set_map_list_to_set_L (SA:=Pset)) in Hx.
+        set_solver.
+      }
+      unfold Pmap_map.
+      enough (_ !! _ = None) as -> by done.
+      apply not_elem_of_list_to_map.
+      rewrite <- vec_to_list_map, fst_vzip, vec_to_list_map; set_solver.
+    }
+    1:{
+      instantiate (1:= (list_to_set (vmap (bcons true) (inputs scohg)))).
+      apply set_eq; intros k.
+      rewrite elem_of_list_to_set, elem_of_map.
+      setoid_rewrite elem_of_list_to_set.
+      rewrite Vector.map_map.
+      setoid_rewrite elem_of_vlookup.
+
+      split.
+      - intros (_ & -> & (i & <-)).
+        exists i.
+        symmetry.
+        unfold Pmap_map.
+        eenough (_ !! _ = Some _) as -> by done.
+        apply elem_of_list_to_map.
+        + rewrite <- vec_to_list_map, fst_vzip, vec_to_list_map, vec_to_list_seq.
+          apply (NoDup_fmap _), NoDup_seq.
+        + apply elem_of_vlookup.
+          exists i.
+          rewrite vlookup_zip_with.
+          done.
+      - intros (i & <-).
+        eexists.
+        split; [|exists i; done].
+        symmetry.
+        unfold Pmap_map.
+        eenough (_ !! _ = Some _) as -> by done.
+        apply elem_of_list_to_map.
+        + rewrite <- vec_to_list_map, fst_vzip, vec_to_list_map, vec_to_list_seq.
+          apply (NoDup_fmap _), NoDup_seq.
+        + apply elem_of_vlookup.
+          exists i.
+          rewrite vlookup_zip_with.
+          done.
+    }
+    set_solver.
+Qed.
+
+
+Lemma compose_sized_graphs_id_sized_graph_l {T n m} (scohg : SizedCospanHyperGraph N T n m) :
+  compose_sized_graphs (id_sized_graph n) scohg ≡ᵢ scohg.
+Proof.
+  rewrite compose_sized_graphs_id_sized_graph_l_aux.
+  rewrite <- sized_iso_relabel_reindex; [done|apply _..].
+Qed.
+
+Lemma stack_sized_graphs_id_sized_graph {T} n m :
+  sized_isomorphic (T:=T) (stack_sized_graphs (id_sized_graph n) (id_sized_graph m))
+    (id_sized_graph (n + m)).
+Proof.
+  symmetry.
+  apply sized_isomorphic_exists.
+  exists (fun i => if decide (pos_to_nat_pred i < n) then i~0 else (pos_sub_N i (N.of_nat n))~1), id.
+  split_and!.
+  - intros i j; do 2 case_decide; lia.
+  - apply _.
+  - eenough (Hen : _) by (apply scohg_ext; [reflexivity|..]; apply Hen).
+    cbn.
+    apply vec_eq.
+    intros i.
+    induction i as [i|i] using fin_add_inv.
+    + rewrite lookup_vapp_L.
+      rewrite 4 vlookup_map, 2 vlookup_seq.
+      pose proof (fin_to_nat_lt i).
+      rewrite fin_to_nat_L.
+      case_decide; [|lia].
+      done.
+    + rewrite lookup_vapp_R.
+      rewrite 4 vlookup_map, 2 vlookup_seq.
+      pose proof (fin_to_nat_lt i).
+      rewrite fin_to_nat_R.
+      case_decide; lia.
+Qed.
+
+ *)
+
+End StackCompose.
